BIL.thy
@@ -2,6 +2,12 @@ theory BIL
   imports Program_Model
 begin
 
+lemma \<Gamma>_val_type_implies_type_t:
+  assumes \<open>\<Gamma> \<turnstile> v :: t\<close>
+    shows \<open>type v = t\<close>
+  using assms by (induct rule: typing_expression_val_induct, auto)
+
+
 (* TODO hide consts etc... here *)
 
 end
