Expression_Semantics.thy
@@ -1,5 +1,5 @@
 theory Expression_Semantics
-  imports Instruction_Syntax
+  imports Instruction_Syntax Typing
 begin
 
 fun 
@@ -9,109 +9,554 @@ where
   \<open>type (Immediate w) = Imm (bits w)\<close> | 
   \<open>type (Unknown str t) = t\<close>
 
+lemma \<Gamma>_val_type:
+  assumes \<open>\<Gamma> \<turnstile> v :: t\<close>
+    shows \<open>type v = t\<close>
+  using assms apply (induct v, simp_all)
+  using typing_expression_val.elims(2) apply fastforce
+  by (metis Type.exhaust \<Gamma>_val_imm_not_storage typing_val_storage)
+
+lemma \<Gamma>_type_val:
+  assumes \<open>type v = t\<close>
+      and \<open>\<Gamma> is ok\<close> and \<open>t is ok\<close>
+      and \<open>\<forall>mem sz\<^sub>m\<^sub>e\<^sub>m w v' sz\<^sub>a\<^sub>d\<^sub>d\<^sub>r. v = (mem[w \<leftarrow> v', sz\<^sub>m\<^sub>e\<^sub>m])
+              \<longrightarrow> (\<Gamma> \<turnstile> v' :: (Imm sz\<^sub>m\<^sub>e\<^sub>m)) \<and> (\<Gamma> \<turnstile> mem :: (Mem sz\<^sub>a\<^sub>d\<^sub>d\<^sub>r sz\<^sub>m\<^sub>e\<^sub>m))\<close>
+    shows \<open>\<Gamma> \<turnstile> v :: t\<close>
+  using assms apply (cases v, auto)
+  apply (case_tac x1, auto)
+  by (case_tac x32, auto)
+
+
+
 definition 
   succ :: \<open>word \<Rightarrow> word\<close>
 where
-  \<open>succ w\<^sub>1 = w\<^sub>1 +\<^sub>b\<^sub>v (1 \<Colon> bits w\<^sub>1)\<close>
+  \<open>succ w\<^sub>1 = w\<^sub>1 +\<^sub>b\<^sub>v (1 \<Colon> (bits w\<^sub>1))\<close>
 
 lemma SUCC: \<open>succ (num \<Colon> sz) = (num \<Colon> sz) +\<^sub>b\<^sub>v (1 \<Colon> sz)\<close>
   by (simp add: succ_def)
 
-fun
-  load_val :: \<open>val \<Rightarrow> word \<Rightarrow> val\<close>
-where 
-  \<open>load_val (Storage v w v' _) w' = (if w = w' then v' else load_val v w')\<close> |
-  \<open>load_val (Unknown str (Mem _ sz)) _ = Unknown str (Imm sz)\<close>
+text \<open>Confirmation Report lemmas\<close>
 
-lemma load_val_next: 
-  assumes \<open>w \<noteq> w'\<close>
-    shows \<open>load_val (Storage v w v' sz) w' = load_val v w'\<close>
+fun
+  load :: \<open>val \<Rightarrow> word \<Rightarrow> nat \<Rightarrow> Endian \<Rightarrow> val\<close>
+where
+  \<open>load (mem[w\<^sub>m\<^sub>e\<^sub>m \<leftarrow> v\<^sub>m\<^sub>e\<^sub>m, sz\<^sub>m\<^sub>e\<^sub>m]) w\<^sub>a\<^sub>d\<^sub>d\<^sub>r sz\<^sub>v\<^sub>a\<^sub>l en = (
+    if sz\<^sub>m\<^sub>e\<^sub>m > 0 \<and> sz\<^sub>v\<^sub>a\<^sub>l > sz\<^sub>m\<^sub>e\<^sub>m then
+      let 
+        sz\<^sub>v\<^sub>a\<^sub>l' :: nat = (sz\<^sub>v\<^sub>a\<^sub>l - sz\<^sub>m\<^sub>e\<^sub>m);
+        w\<^sub>a\<^sub>d\<^sub>d\<^sub>r' :: word = succ w\<^sub>a\<^sub>d\<^sub>d\<^sub>r;
+        v\<^sub>v\<^sub>a\<^sub>l :: val = load (mem[w\<^sub>m\<^sub>e\<^sub>m \<leftarrow> v\<^sub>m\<^sub>e\<^sub>m, sz\<^sub>m\<^sub>e\<^sub>m]) w\<^sub>a\<^sub>d\<^sub>d\<^sub>r sz\<^sub>m\<^sub>e\<^sub>m en;
+        v\<^sub>c\<^sub>o\<^sub>n\<^sub>c\<^sub>a\<^sub>t :: val = load (mem[w\<^sub>m\<^sub>e\<^sub>m \<leftarrow> v\<^sub>m\<^sub>e\<^sub>m, sz\<^sub>m\<^sub>e\<^sub>m]) w\<^sub>a\<^sub>d\<^sub>d\<^sub>r' sz\<^sub>v\<^sub>a\<^sub>l' en
+      in
+        case v\<^sub>v\<^sub>a\<^sub>l of Immediate w\<^sub>v\<^sub>a\<^sub>l \<Rightarrow> (
+          case v\<^sub>c\<^sub>o\<^sub>n\<^sub>c\<^sub>a\<^sub>t of Immediate w\<^sub>c\<^sub>o\<^sub>n\<^sub>c\<^sub>a\<^sub>t \<Rightarrow> (
+            case en of
+              be \<Rightarrow> Immediate (w\<^sub>v\<^sub>a\<^sub>l \<cdot> w\<^sub>c\<^sub>o\<^sub>n\<^sub>c\<^sub>a\<^sub>t) |
+              el \<Rightarrow> Immediate (w\<^sub>c\<^sub>o\<^sub>n\<^sub>c\<^sub>a\<^sub>t \<cdot> w\<^sub>v\<^sub>a\<^sub>l)
+          ) | unknown[str]: _ \<Rightarrow> unknown[str]: (Imm sz\<^sub>v\<^sub>a\<^sub>l)
+        ) | unknown[str]: _ \<Rightarrow> unknown[str]: (Imm sz\<^sub>v\<^sub>a\<^sub>l)
+    else (
+      if w\<^sub>m\<^sub>e\<^sub>m = w\<^sub>a\<^sub>d\<^sub>d\<^sub>r then v\<^sub>m\<^sub>e\<^sub>m 
+      else load mem w\<^sub>a\<^sub>d\<^sub>d\<^sub>r sz\<^sub>v\<^sub>a\<^sub>l en
+    )
+  )\<close> |
+  \<open>load (unknown[str]: _) _ sz\<^sub>v\<^sub>a\<^sub>l _ = unknown[str]: (Imm sz\<^sub>v\<^sub>a\<^sub>l) \<close> |
+  \<open>load (Immediate _) _ _ _ = undefined\<close>
+
+lemma load_mem_simps: 
+  assumes \<open>v = (mem[w\<^sub>m\<^sub>e\<^sub>m \<leftarrow> v\<^sub>m\<^sub>e\<^sub>m, sz\<^sub>m\<^sub>e\<^sub>m])\<close> 
+    shows \<open>load v w\<^sub>a\<^sub>d\<^sub>d\<^sub>r sz\<^sub>v\<^sub>a\<^sub>l en = (
+    if sz\<^sub>m\<^sub>e\<^sub>m > 0 \<and> sz\<^sub>v\<^sub>a\<^sub>l > sz\<^sub>m\<^sub>e\<^sub>m then
+      let 
+        sz\<^sub>v\<^sub>a\<^sub>l' :: nat = (sz\<^sub>v\<^sub>a\<^sub>l - sz\<^sub>m\<^sub>e\<^sub>m);
+        w\<^sub>a\<^sub>d\<^sub>d\<^sub>r' :: word = succ w\<^sub>a\<^sub>d\<^sub>d\<^sub>r;
+        v\<^sub>v\<^sub>a\<^sub>l :: val = load (mem[w\<^sub>m\<^sub>e\<^sub>m \<leftarrow> v\<^sub>m\<^sub>e\<^sub>m, sz\<^sub>m\<^sub>e\<^sub>m]) w\<^sub>a\<^sub>d\<^sub>d\<^sub>r sz\<^sub>m\<^sub>e\<^sub>m en;
+        v\<^sub>c\<^sub>o\<^sub>n\<^sub>c\<^sub>a\<^sub>t :: val = load (mem[w\<^sub>m\<^sub>e\<^sub>m \<leftarrow> v\<^sub>m\<^sub>e\<^sub>m, sz\<^sub>m\<^sub>e\<^sub>m]) w\<^sub>a\<^sub>d\<^sub>d\<^sub>r' sz\<^sub>v\<^sub>a\<^sub>l' en
+      in
+        case v\<^sub>v\<^sub>a\<^sub>l of Immediate w\<^sub>v\<^sub>a\<^sub>l \<Rightarrow> (
+          case v\<^sub>c\<^sub>o\<^sub>n\<^sub>c\<^sub>a\<^sub>t of Immediate w\<^sub>c\<^sub>o\<^sub>n\<^sub>c\<^sub>a\<^sub>t \<Rightarrow> (
+            case en of
+              be \<Rightarrow> Immediate (w\<^sub>v\<^sub>a\<^sub>l \<cdot> w\<^sub>c\<^sub>o\<^sub>n\<^sub>c\<^sub>a\<^sub>t) |
+              el \<Rightarrow> Immediate (w\<^sub>c\<^sub>o\<^sub>n\<^sub>c\<^sub>a\<^sub>t \<cdot> w\<^sub>v\<^sub>a\<^sub>l)
+          ) | unknown[str]: _ \<Rightarrow> unknown[str]: (Imm sz\<^sub>v\<^sub>a\<^sub>l)
+        ) | unknown[str]: _ \<Rightarrow> unknown[str]: (Imm sz\<^sub>v\<^sub>a\<^sub>l)
+    else (
+      if w\<^sub>m\<^sub>e\<^sub>m = w\<^sub>a\<^sub>d\<^sub>d\<^sub>r then v\<^sub>m\<^sub>e\<^sub>m 
+      else load mem w\<^sub>a\<^sub>d\<^sub>d\<^sub>r sz\<^sub>v\<^sub>a\<^sub>l en
+    )
+  )\<close>
   using assms by auto
 
+lemma load: \<open>v' = load (v[w \<leftarrow> v', sz]) w sz en\<close>
+  by auto
+
+lemma load_neq:
+  assumes \<open>v'' = load v w' sz\<^sub>v\<^sub>a\<^sub>l en\<close> and \<open>w \<noteq> w'\<close> and \<open>type v = Mem sz\<^sub>a\<^sub>d\<^sub>d\<^sub>r sz\<^sub>v\<^sub>a\<^sub>l\<close>
+    shows \<open>v'' = load (Storage v w v' sz\<^sub>v\<^sub>a\<^sub>l) w' sz\<^sub>v\<^sub>a\<^sub>l en\<close>
+  using assms by auto
+
+lemma load_unk: \<open>(unknown[str]: (Imm sz)) = load (unknown[str]: t) w sz en\<close>
+  by auto
+
+lemma load_unk_base:
+  assumes \<open>type v = Mem sz\<^sub>a\<^sub>d\<^sub>d\<^sub>r sz\<^sub>m\<^sub>e\<^sub>m\<close> and \<open>sz\<^sub>m\<^sub>e\<^sub>m > 0\<close> and \<open>sz\<^sub>v\<^sub>a\<^sub>l > sz\<^sub>m\<^sub>e\<^sub>m\<close>
+      and \<open>(unknown[str]: (Imm sz\<^sub>m\<^sub>e\<^sub>m)) = load v w sz\<^sub>m\<^sub>e\<^sub>m en\<close>
+    shows \<open>(unknown[str]: (Imm sz\<^sub>v\<^sub>a\<^sub>l)) = load v w sz\<^sub>v\<^sub>a\<^sub>l en\<close>
+  apply (cases v)
+  using assms(1) apply simp
+  using assms(4) apply fastforce
+  apply (frule_tac w\<^sub>a\<^sub>d\<^sub>d\<^sub>r=w and sz\<^sub>v\<^sub>a\<^sub>l=sz\<^sub>v\<^sub>a\<^sub>l and en=en in load_mem_simps)
+  using assms apply (auto simp del: load.simps)
+  apply auto[1]  
+  by (metis val.simps(11))
+
+lemma load_unk_rec:
+  assumes \<open>type v = Mem sz\<^sub>a\<^sub>d\<^sub>d\<^sub>r sz\<^sub>m\<^sub>e\<^sub>m\<close> and \<open>sz\<^sub>m\<^sub>e\<^sub>m > 0\<close> and \<open>sz\<^sub>v\<^sub>a\<^sub>l > sz\<^sub>m\<^sub>e\<^sub>m\<close>
+      and \<open>(Immediate w') = load v w sz\<^sub>m\<^sub>e\<^sub>m en\<close>
+      and \<open>(unknown[str]: (Imm (sz\<^sub>v\<^sub>a\<^sub>l - sz\<^sub>m\<^sub>e\<^sub>m))) = load v (succ w) (sz\<^sub>v\<^sub>a\<^sub>l - sz\<^sub>m\<^sub>e\<^sub>m) en\<close>
+    shows \<open>(unknown[str]: (Imm sz\<^sub>v\<^sub>a\<^sub>l)) = load v w sz\<^sub>v\<^sub>a\<^sub>l en\<close>
+  apply (cases v)
+  using assms(1) apply fastforce
+  using assms(5) apply fastforce
+  apply (frule_tac w\<^sub>a\<^sub>d\<^sub>d\<^sub>r=w and sz\<^sub>v\<^sub>a\<^sub>l=sz\<^sub>v\<^sub>a\<^sub>l and en=en in load_mem_simps)
+  using assms apply (auto simp del: load.simps)
+  by (metis val.simps(10) val.simps(11))
+
+lemma load_be:
+  assumes \<open>type v = Mem sz\<^sub>a\<^sub>d\<^sub>d\<^sub>r sz\<^sub>m\<^sub>e\<^sub>m\<close> and \<open>sz\<^sub>m\<^sub>e\<^sub>m > 0\<close> and \<open>sz\<^sub>v\<^sub>a\<^sub>l > sz\<^sub>m\<^sub>e\<^sub>m\<close>
+      and \<open>Immediate w\<^sub>1 = load v w sz\<^sub>m\<^sub>e\<^sub>m be\<close>
+      and \<open>Immediate w\<^sub>2 = load v (succ w) (sz\<^sub>v\<^sub>a\<^sub>l - sz\<^sub>m\<^sub>e\<^sub>m) be\<close>
+      and \<open>w' = w\<^sub>1 \<cdot> w\<^sub>2\<close>
+    shows \<open>Immediate w' = load v w sz\<^sub>v\<^sub>a\<^sub>l be\<close>
+  apply (cases v)
+  using assms(1) apply fastforce
+  using assms(5) apply fastforce
+  apply (frule_tac w\<^sub>a\<^sub>d\<^sub>d\<^sub>r=w and sz\<^sub>v\<^sub>a\<^sub>l=sz\<^sub>v\<^sub>a\<^sub>l and en=be in load_mem_simps)
+  using assms apply (auto simp del: load.simps)
+  by (metis Endian.simps(4) assms(6) val.simps(10))
+
+lemma load_el:
+  assumes \<open>type v = Mem sz\<^sub>a\<^sub>d\<^sub>d\<^sub>r sz\<^sub>m\<^sub>e\<^sub>m\<close> and \<open>sz\<^sub>m\<^sub>e\<^sub>m > 0\<close> and \<open>sz\<^sub>v\<^sub>a\<^sub>l > sz\<^sub>m\<^sub>e\<^sub>m\<close>
+      and \<open>Immediate w\<^sub>1 = load v w sz\<^sub>m\<^sub>e\<^sub>m el\<close>
+      and \<open>Immediate w\<^sub>2 = load v (succ w) (sz\<^sub>v\<^sub>a\<^sub>l - sz\<^sub>m\<^sub>e\<^sub>m) el\<close>
+      and \<open>w' = w\<^sub>2 \<cdot> w\<^sub>1\<close>
+    shows \<open>Immediate w' = load v w sz\<^sub>v\<^sub>a\<^sub>l el\<close>
+  apply (cases v)
+  using assms(1) apply fastforce
+  using assms(5) apply fastforce
+  apply (frule_tac w\<^sub>a\<^sub>d\<^sub>d\<^sub>r=w and sz\<^sub>v\<^sub>a\<^sub>l=sz\<^sub>v\<^sub>a\<^sub>l and en=el in load_mem_simps)
+  using assms apply (auto simp del: load.simps)
+  by (metis Endian.simps(3) assms(6) val.simps(10))
+
+
+
+subsubsection \<open>Store\<close>
+
 fun
-  load_val_be :: \<open>val \<Rightarrow> word \<Rightarrow> nat \<Rightarrow> val\<close>
-where 
-  \<open>load_val_be mem w 0 = load_val mem w\<close> |
-  \<open>load_val_be mem w (Suc n) = (
-    case load_val_be mem (succ w) n of Immediate w\<^sub>c\<^sub>o\<^sub>n\<^sub>c\<^sub>a\<^sub>t \<Rightarrow> (
-      case load_val mem w of Immediate w\<^sub>v\<^sub>a\<^sub>l \<Rightarrow> Immediate (w\<^sub>v\<^sub>a\<^sub>l \<cdot> w\<^sub>c\<^sub>o\<^sub>n\<^sub>c\<^sub>a\<^sub>t)
-      | Unknown str (Imm sz) \<Rightarrow> Unknown str (Imm (bits w\<^sub>c\<^sub>o\<^sub>n\<^sub>c\<^sub>a\<^sub>t + sz)))
-    | Unknown str (Imm sz) \<Rightarrow> Unknown str (Imm sz)
+  store :: \<open>val \<Rightarrow> word \<Rightarrow> val \<Rightarrow> nat \<Rightarrow> Endian \<Rightarrow> val\<close>
+where
+  \<open>store mem w\<^sub>a\<^sub>d\<^sub>d\<^sub>r v\<^sub>v\<^sub>a\<^sub>l sz\<^sub>v\<^sub>a\<^sub>l en = (
+    case type mem of Mem _ sz\<^sub>m\<^sub>e\<^sub>m \<Rightarrow> (
+      if sz\<^sub>m\<^sub>e\<^sub>m = 0 then undefined
+      else if sz\<^sub>v\<^sub>a\<^sub>l < sz\<^sub>m\<^sub>e\<^sub>m then undefined
+      else if sz\<^sub>v\<^sub>a\<^sub>l > sz\<^sub>m\<^sub>e\<^sub>m then
+        let 
+          sz\<^sub>v\<^sub>a\<^sub>l' :: nat = (sz\<^sub>v\<^sub>a\<^sub>l - sz\<^sub>m\<^sub>e\<^sub>m);
+          w\<^sub>a\<^sub>d\<^sub>d\<^sub>r' :: word = succ w\<^sub>a\<^sub>d\<^sub>d\<^sub>r 
+        in 
+          case v\<^sub>v\<^sub>a\<^sub>l of Immediate w\<^sub>v\<^sub>a\<^sub>l \<Rightarrow> (
+            let 
+              w\<^sub>v\<^sub>a\<^sub>l\<^sub>_\<^sub>c\<^sub>o\<^sub>n\<^sub>c\<^sub>a\<^sub>t :: word = (case en of 
+                be \<Rightarrow> ext w\<^sub>v\<^sub>a\<^sub>l \<sim> hi : sz\<^sub>v\<^sub>a\<^sub>l' \<sim> lo : 0 |
+                el \<Rightarrow> ext w\<^sub>v\<^sub>a\<^sub>l \<sim> hi : sz\<^sub>v\<^sub>a\<^sub>l \<sim> lo : sz\<^sub>m\<^sub>e\<^sub>m);
+              w\<^sub>v\<^sub>a\<^sub>l\<^sub>_\<^sub>v\<^sub>a\<^sub>l :: word = (case en of 
+                be \<Rightarrow> ext w\<^sub>v\<^sub>a\<^sub>l \<sim> hi : sz\<^sub>v\<^sub>a\<^sub>l \<sim> lo : sz\<^sub>v\<^sub>a\<^sub>l' | 
+                el \<Rightarrow> ext w\<^sub>v\<^sub>a\<^sub>l \<sim> hi : sz\<^sub>m\<^sub>e\<^sub>m \<sim> lo : 0); 
+              mem' :: val = mem[w\<^sub>a\<^sub>d\<^sub>d\<^sub>r \<leftarrow> (Immediate w\<^sub>v\<^sub>a\<^sub>l\<^sub>_\<^sub>v\<^sub>a\<^sub>l), sz\<^sub>m\<^sub>e\<^sub>m]
+            in
+              store mem' w\<^sub>a\<^sub>d\<^sub>d\<^sub>r' (Immediate w\<^sub>v\<^sub>a\<^sub>l\<^sub>_\<^sub>c\<^sub>o\<^sub>n\<^sub>c\<^sub>a\<^sub>t) sz\<^sub>v\<^sub>a\<^sub>l' en
+        ) | Unknown str t \<Rightarrow> (
+          let mem' :: val = mem[w\<^sub>a\<^sub>d\<^sub>d\<^sub>r \<leftarrow> (Unknown str (Imm sz\<^sub>m\<^sub>e\<^sub>m)), sz\<^sub>m\<^sub>e\<^sub>m] in
+            store mem' w\<^sub>a\<^sub>d\<^sub>d\<^sub>r' (Unknown str (Imm sz\<^sub>v\<^sub>a\<^sub>l')) sz\<^sub>v\<^sub>a\<^sub>l' en
+        )
+      else (mem[w\<^sub>a\<^sub>d\<^sub>d\<^sub>r \<leftarrow> v\<^sub>v\<^sub>a\<^sub>l, sz\<^sub>m\<^sub>e\<^sub>m])
+    )
   )\<close>
 
-fun
-  load_val_el :: \<open>val \<Rightarrow> word \<Rightarrow> nat \<Rightarrow> val\<close>
-where 
-  \<open>load_val_el mem w 0 = load_val mem w\<close> |
-  \<open>load_val_el mem w (Suc n) = (
-    case load_val_el mem (succ w) n of Immediate w\<^sub>c\<^sub>o\<^sub>n\<^sub>c\<^sub>a\<^sub>t \<Rightarrow> (
-      case load_val mem w of Immediate w\<^sub>v\<^sub>a\<^sub>l \<Rightarrow> Immediate (w\<^sub>c\<^sub>o\<^sub>n\<^sub>c\<^sub>a\<^sub>t \<cdot> w\<^sub>v\<^sub>a\<^sub>l)
-      | v \<Rightarrow> v)
-    | v \<Rightarrow> v
-  )\<close>
+thm store.induct
 
 fun
-  load_val_en :: \<open>val \<Rightarrow> nat \<Rightarrow> word \<Rightarrow> nat \<Rightarrow> Endian \<Rightarrow> val\<close>
-where 
-  \<open>load_val_en mem sz\<^sub>m\<^sub>e\<^sub>m w sz\<^sub>v\<^sub>a\<^sub>l be =
-    load_val_be mem w (sz\<^sub>v\<^sub>a\<^sub>l div sz\<^sub>m\<^sub>e\<^sub>m - 1)
-  \<close> |
-  \<open>load_val_en mem sz\<^sub>m\<^sub>e\<^sub>m w sz\<^sub>v\<^sub>a\<^sub>l el =
-    load_val_el mem w (sz\<^sub>v\<^sub>a\<^sub>l div sz\<^sub>m\<^sub>e\<^sub>m - 1)\<close>
+  store' :: \<open>val \<Rightarrow> word \<Rightarrow> val \<Rightarrow> nat \<Rightarrow> Endian \<Rightarrow> val\<close>
+where
+  \<open>store' (unknown[vstr]: (Mem sz\<^sub>a\<^sub>d\<^sub>d\<^sub>r sz\<^sub>m\<^sub>e\<^sub>m)) w\<^sub>a\<^sub>d\<^sub>d\<^sub>r (Immediate w\<^sub>v\<^sub>a\<^sub>l) sz\<^sub>v\<^sub>a\<^sub>l el = (
+      if bits w\<^sub>a\<^sub>d\<^sub>d\<^sub>r \<noteq> sz\<^sub>a\<^sub>d\<^sub>d\<^sub>r then undefined
+      else if bits w\<^sub>v\<^sub>a\<^sub>l \<noteq> sz\<^sub>v\<^sub>a\<^sub>l then undefined
+      else if sz\<^sub>m\<^sub>e\<^sub>m = 0 then undefined
+      else if sz\<^sub>v\<^sub>a\<^sub>l < sz\<^sub>m\<^sub>e\<^sub>m then undefined
+      else if sz\<^sub>v\<^sub>a\<^sub>l > sz\<^sub>m\<^sub>e\<^sub>m then
+        store' ((unknown[vstr]: (Mem sz\<^sub>a\<^sub>d\<^sub>d\<^sub>r sz\<^sub>m\<^sub>e\<^sub>m))[w\<^sub>a\<^sub>d\<^sub>d\<^sub>r \<leftarrow> (Immediate ((ext w\<^sub>v\<^sub>a\<^sub>l \<sim> hi : sz\<^sub>m\<^sub>e\<^sub>m \<sim> lo : 0))), sz\<^sub>m\<^sub>e\<^sub>m]) (succ w\<^sub>a\<^sub>d\<^sub>d\<^sub>r ) (Immediate (ext w\<^sub>v\<^sub>a\<^sub>l \<sim> hi : sz\<^sub>v\<^sub>a\<^sub>l \<sim> lo : sz\<^sub>m\<^sub>e\<^sub>m)) (sz\<^sub>v\<^sub>a\<^sub>l - sz\<^sub>m\<^sub>e\<^sub>m) el
+      else ((unknown[vstr]: (Mem sz\<^sub>a\<^sub>d\<^sub>d\<^sub>r sz\<^sub>m\<^sub>e\<^sub>m))[w\<^sub>a\<^sub>d\<^sub>d\<^sub>r \<leftarrow> (Immediate w\<^sub>v\<^sub>a\<^sub>l), sz\<^sub>m\<^sub>e\<^sub>m])
+  )\<close> |
+  \<open>store' (unknown[vstr]: (Mem sz\<^sub>a\<^sub>d\<^sub>d\<^sub>r sz\<^sub>m\<^sub>e\<^sub>m)) w\<^sub>a\<^sub>d\<^sub>d\<^sub>r (Immediate w\<^sub>v\<^sub>a\<^sub>l) sz\<^sub>v\<^sub>a\<^sub>l be = (
+      if bits w\<^sub>a\<^sub>d\<^sub>d\<^sub>r \<noteq> sz\<^sub>a\<^sub>d\<^sub>d\<^sub>r then undefined
+      else if bits w\<^sub>v\<^sub>a\<^sub>l \<noteq> sz\<^sub>v\<^sub>a\<^sub>l then undefined
+      else if sz\<^sub>m\<^sub>e\<^sub>m = 0 then undefined
+      else if sz\<^sub>v\<^sub>a\<^sub>l < sz\<^sub>m\<^sub>e\<^sub>m then undefined
+      else if sz\<^sub>v\<^sub>a\<^sub>l > sz\<^sub>m\<^sub>e\<^sub>m then
+        store' ((unknown[vstr]: (Mem sz\<^sub>a\<^sub>d\<^sub>d\<^sub>r sz\<^sub>m\<^sub>e\<^sub>m))[w\<^sub>a\<^sub>d\<^sub>d\<^sub>r \<leftarrow> (Immediate (ext w\<^sub>v\<^sub>a\<^sub>l \<sim> hi : sz\<^sub>v\<^sub>a\<^sub>l \<sim> lo : (sz\<^sub>v\<^sub>a\<^sub>l - sz\<^sub>m\<^sub>e\<^sub>m))), sz\<^sub>m\<^sub>e\<^sub>m]) (succ w\<^sub>a\<^sub>d\<^sub>d\<^sub>r) (Immediate (ext w\<^sub>v\<^sub>a\<^sub>l \<sim> hi : (sz\<^sub>v\<^sub>a\<^sub>l - sz\<^sub>m\<^sub>e\<^sub>m) \<sim> lo : 0)) (sz\<^sub>v\<^sub>a\<^sub>l - sz\<^sub>m\<^sub>e\<^sub>m) be        
+      else ((unknown[vstr]: (Mem sz\<^sub>a\<^sub>d\<^sub>d\<^sub>r sz\<^sub>m\<^sub>e\<^sub>m))[w\<^sub>a\<^sub>d\<^sub>d\<^sub>r \<leftarrow> (Immediate w\<^sub>v\<^sub>a\<^sub>l), sz\<^sub>m\<^sub>e\<^sub>m])
+  )\<close> |
+  \<open>store' (unknown[vstr]: (Mem sz\<^sub>a\<^sub>d\<^sub>d\<^sub>r sz\<^sub>m\<^sub>e\<^sub>m)) w\<^sub>a\<^sub>d\<^sub>d\<^sub>r (Unknown str (Imm sz)) sz\<^sub>v\<^sub>a\<^sub>l en = (
+      if bits w\<^sub>a\<^sub>d\<^sub>d\<^sub>r \<noteq> sz\<^sub>a\<^sub>d\<^sub>d\<^sub>r then undefined
+      else if sz \<noteq> sz\<^sub>v\<^sub>a\<^sub>l then undefined
+      else if sz\<^sub>m\<^sub>e\<^sub>m = 0 then undefined
+      else if sz\<^sub>v\<^sub>a\<^sub>l < sz\<^sub>m\<^sub>e\<^sub>m then undefined
+      else if sz\<^sub>v\<^sub>a\<^sub>l > sz\<^sub>m\<^sub>e\<^sub>m then
+        store' ((unknown[vstr]: (Mem sz\<^sub>a\<^sub>d\<^sub>d\<^sub>r sz\<^sub>m\<^sub>e\<^sub>m))[w\<^sub>a\<^sub>d\<^sub>d\<^sub>r \<leftarrow> (Unknown str (Imm sz\<^sub>m\<^sub>e\<^sub>m)), sz\<^sub>m\<^sub>e\<^sub>m]) (succ w\<^sub>a\<^sub>d\<^sub>d\<^sub>r) (Unknown str (Imm (sz\<^sub>v\<^sub>a\<^sub>l - sz\<^sub>m\<^sub>e\<^sub>m))) (sz\<^sub>v\<^sub>a\<^sub>l - sz\<^sub>m\<^sub>e\<^sub>m) en        
+      else ((unknown[vstr]: (Mem sz\<^sub>a\<^sub>d\<^sub>d\<^sub>r sz\<^sub>m\<^sub>e\<^sub>m))[w\<^sub>a\<^sub>d\<^sub>d\<^sub>r \<leftarrow> (Unknown str (Imm sz)), sz\<^sub>m\<^sub>e\<^sub>m])
+  )\<close> |
+  \<open>store' (memR[wR \<leftarrow> vR, sz\<^sub>m\<^sub>e\<^sub>m]) w\<^sub>a\<^sub>d\<^sub>d\<^sub>r (Immediate w\<^sub>v\<^sub>a\<^sub>l) sz\<^sub>v\<^sub>a\<^sub>l be = (
+      if bits w\<^sub>a\<^sub>d\<^sub>d\<^sub>r \<noteq> bits wR then undefined
+      else if bits w\<^sub>v\<^sub>a\<^sub>l \<noteq> sz\<^sub>v\<^sub>a\<^sub>l then undefined
+      else if sz\<^sub>m\<^sub>e\<^sub>m = 0 then undefined
+      else if sz\<^sub>v\<^sub>a\<^sub>l < sz\<^sub>m\<^sub>e\<^sub>m then undefined
+      else if sz\<^sub>v\<^sub>a\<^sub>l > sz\<^sub>m\<^sub>e\<^sub>m then
+        store' ((memR[wR \<leftarrow> vR, sz\<^sub>m\<^sub>e\<^sub>m])[w\<^sub>a\<^sub>d\<^sub>d\<^sub>r \<leftarrow> (Immediate (ext w\<^sub>v\<^sub>a\<^sub>l \<sim> hi : sz\<^sub>v\<^sub>a\<^sub>l \<sim> lo : (sz\<^sub>v\<^sub>a\<^sub>l - sz\<^sub>m\<^sub>e\<^sub>m))), sz\<^sub>m\<^sub>e\<^sub>m]) (succ w\<^sub>a\<^sub>d\<^sub>d\<^sub>r) (Immediate (ext w\<^sub>v\<^sub>a\<^sub>l \<sim> hi : (sz\<^sub>v\<^sub>a\<^sub>l - sz\<^sub>m\<^sub>e\<^sub>m) \<sim> lo : 0)) (sz\<^sub>v\<^sub>a\<^sub>l - sz\<^sub>m\<^sub>e\<^sub>m) be
+      else ((memR[wR \<leftarrow> vR, sz\<^sub>m\<^sub>e\<^sub>m])[w\<^sub>a\<^sub>d\<^sub>d\<^sub>r \<leftarrow> (Immediate w\<^sub>v\<^sub>a\<^sub>l), sz\<^sub>m\<^sub>e\<^sub>m])
+  )\<close> |
+  \<open>store' (memR[wR \<leftarrow> vR, sz\<^sub>m\<^sub>e\<^sub>m]) w\<^sub>a\<^sub>d\<^sub>d\<^sub>r (Immediate w\<^sub>v\<^sub>a\<^sub>l) sz\<^sub>v\<^sub>a\<^sub>l el = (
+      if bits w\<^sub>a\<^sub>d\<^sub>d\<^sub>r \<noteq> bits wR then undefined
+      else if bits w\<^sub>v\<^sub>a\<^sub>l \<noteq> sz\<^sub>v\<^sub>a\<^sub>l then undefined
+      else if sz\<^sub>m\<^sub>e\<^sub>m = 0 then undefined
+      else if sz\<^sub>v\<^sub>a\<^sub>l < sz\<^sub>m\<^sub>e\<^sub>m then undefined
+      else if sz\<^sub>v\<^sub>a\<^sub>l > sz\<^sub>m\<^sub>e\<^sub>m then
+        store' ((memR[wR \<leftarrow> vR, sz\<^sub>m\<^sub>e\<^sub>m])[w\<^sub>a\<^sub>d\<^sub>d\<^sub>r \<leftarrow> (Immediate (ext w\<^sub>v\<^sub>a\<^sub>l \<sim> hi : sz\<^sub>m\<^sub>e\<^sub>m \<sim> lo : 0)), sz\<^sub>m\<^sub>e\<^sub>m]) (succ w\<^sub>a\<^sub>d\<^sub>d\<^sub>r) (Immediate (ext w\<^sub>v\<^sub>a\<^sub>l \<sim> hi : sz\<^sub>v\<^sub>a\<^sub>l \<sim> lo : sz\<^sub>m\<^sub>e\<^sub>m)) (sz\<^sub>v\<^sub>a\<^sub>l - sz\<^sub>m\<^sub>e\<^sub>m) el
+      else ((memR[wR \<leftarrow> vR, sz\<^sub>m\<^sub>e\<^sub>m])[w\<^sub>a\<^sub>d\<^sub>d\<^sub>r \<leftarrow> (Immediate w\<^sub>v\<^sub>a\<^sub>l), sz\<^sub>m\<^sub>e\<^sub>m])
+  )\<close> |
+  \<open>store' (memR[wR \<leftarrow> vR, sz\<^sub>m\<^sub>e\<^sub>m]) w\<^sub>a\<^sub>d\<^sub>d\<^sub>r (Unknown str (Imm sz)) sz\<^sub>v\<^sub>a\<^sub>l en = (
+      if bits w\<^sub>a\<^sub>d\<^sub>d\<^sub>r \<noteq> bits wR then undefined
+      else if sz \<noteq> sz\<^sub>v\<^sub>a\<^sub>l then undefined
+      else if sz\<^sub>m\<^sub>e\<^sub>m = 0 then undefined
+      else if sz\<^sub>v\<^sub>a\<^sub>l < sz\<^sub>m\<^sub>e\<^sub>m then undefined
+      else if sz\<^sub>v\<^sub>a\<^sub>l > sz\<^sub>m\<^sub>e\<^sub>m then
+        store' ((memR[wR \<leftarrow> vR, sz\<^sub>m\<^sub>e\<^sub>m])[w\<^sub>a\<^sub>d\<^sub>d\<^sub>r \<leftarrow> (Unknown str (Imm sz\<^sub>m\<^sub>e\<^sub>m)), sz\<^sub>m\<^sub>e\<^sub>m]) (succ w\<^sub>a\<^sub>d\<^sub>d\<^sub>r) (Unknown str (Imm (sz\<^sub>v\<^sub>a\<^sub>l - sz\<^sub>m\<^sub>e\<^sub>m))) (sz\<^sub>v\<^sub>a\<^sub>l - sz\<^sub>m\<^sub>e\<^sub>m) en
+      else ((memR[wR \<leftarrow> vR, sz\<^sub>m\<^sub>e\<^sub>m])[w\<^sub>a\<^sub>d\<^sub>d\<^sub>r \<leftarrow> (Unknown str (Imm sz)), sz\<^sub>m\<^sub>e\<^sub>m])
+  )\<close> |
+  \<open>store' _ _ _ _ _ = undefined\<close>
 
-definition
-  store_val :: \<open>val \<Rightarrow> word \<Rightarrow> val \<Rightarrow> nat \<Rightarrow> val\<close>
-where 
-  \<open>store_val mem w v sz\<^sub>m\<^sub>e\<^sub>m = Storage mem w v sz\<^sub>m\<^sub>e\<^sub>m\<close>
+thm store'.induct
+
+(*\<Gamma> \<turnstile> mem :: Mem sz\<^sub>a\<^sub>d\<^sub>d\<^sub>r sz\<^sub>m\<^sub>e\<^sub>m*)
+
+lemma store_inducts[consumes 1]:
+  assumes \<open>v' = store mem w\<^sub>a\<^sub>d\<^sub>d\<^sub>r v\<^sub>v\<^sub>a\<^sub>l sz\<^sub>v\<^sub>a\<^sub>l en\<close>
+      and \<open>\<And>sz\<^sub>a\<^sub>d\<^sub>d\<^sub>r sz\<^sub>m\<^sub>e\<^sub>m w\<^sub>v\<^sub>a\<^sub>l. \<lbrakk>type mem = Mem sz\<^sub>a\<^sub>d\<^sub>d\<^sub>r sz\<^sub>m\<^sub>e\<^sub>m; sz\<^sub>m\<^sub>e\<^sub>m \<noteq> 0; sz\<^sub>v\<^sub>a\<^sub>l > sz\<^sub>m\<^sub>e\<^sub>m; 
+              v\<^sub>v\<^sub>a\<^sub>l = Immediate w\<^sub>v\<^sub>a\<^sub>l; en = be; v' = (
+            let 
+              w\<^sub>v\<^sub>a\<^sub>l\<^sub>_\<^sub>c\<^sub>o\<^sub>n\<^sub>c\<^sub>a\<^sub>t :: word = ext w\<^sub>v\<^sub>a\<^sub>l \<sim> hi : (sz\<^sub>v\<^sub>a\<^sub>l - sz\<^sub>m\<^sub>e\<^sub>m) \<sim> lo : 0;
+              w\<^sub>v\<^sub>a\<^sub>l\<^sub>_\<^sub>v\<^sub>a\<^sub>l :: word = ext w\<^sub>v\<^sub>a\<^sub>l \<sim> hi : sz\<^sub>v\<^sub>a\<^sub>l \<sim> lo : (sz\<^sub>v\<^sub>a\<^sub>l - sz\<^sub>m\<^sub>e\<^sub>m)
+            in
+              store (mem[w\<^sub>a\<^sub>d\<^sub>d\<^sub>r \<leftarrow> (Immediate w\<^sub>v\<^sub>a\<^sub>l\<^sub>_\<^sub>v\<^sub>a\<^sub>l), sz\<^sub>m\<^sub>e\<^sub>m]) (succ w\<^sub>a\<^sub>d\<^sub>d\<^sub>r) (Immediate w\<^sub>v\<^sub>a\<^sub>l\<^sub>_\<^sub>c\<^sub>o\<^sub>n\<^sub>c\<^sub>a\<^sub>t) (sz\<^sub>v\<^sub>a\<^sub>l - sz\<^sub>m\<^sub>e\<^sub>m) be)\<rbrakk> \<Longrightarrow> P mem w\<^sub>a\<^sub>d\<^sub>d\<^sub>r (Immediate w\<^sub>v\<^sub>a\<^sub>l) sz\<^sub>v\<^sub>a\<^sub>l be\<close>
+      and \<open>\<And>sz\<^sub>a\<^sub>d\<^sub>d\<^sub>r sz\<^sub>m\<^sub>e\<^sub>m w\<^sub>v\<^sub>a\<^sub>l. \<lbrakk>type mem = Mem sz\<^sub>a\<^sub>d\<^sub>d\<^sub>r sz\<^sub>m\<^sub>e\<^sub>m; sz\<^sub>m\<^sub>e\<^sub>m \<noteq> 0; sz\<^sub>v\<^sub>a\<^sub>l > sz\<^sub>m\<^sub>e\<^sub>m; 
+              v\<^sub>v\<^sub>a\<^sub>l = Immediate w\<^sub>v\<^sub>a\<^sub>l; en = el; v' = (
+            let 
+              w\<^sub>v\<^sub>a\<^sub>l\<^sub>_\<^sub>c\<^sub>o\<^sub>n\<^sub>c\<^sub>a\<^sub>t :: word = ext w\<^sub>v\<^sub>a\<^sub>l \<sim> hi : sz\<^sub>v\<^sub>a\<^sub>l \<sim> lo : sz\<^sub>m\<^sub>e\<^sub>m;
+              w\<^sub>v\<^sub>a\<^sub>l\<^sub>_\<^sub>v\<^sub>a\<^sub>l :: word = ext w\<^sub>v\<^sub>a\<^sub>l \<sim> hi : sz\<^sub>m\<^sub>e\<^sub>m \<sim> lo : 0
+            in
+              store (mem[w\<^sub>a\<^sub>d\<^sub>d\<^sub>r \<leftarrow> (Immediate w\<^sub>v\<^sub>a\<^sub>l\<^sub>_\<^sub>v\<^sub>a\<^sub>l), sz\<^sub>m\<^sub>e\<^sub>m]) (succ w\<^sub>a\<^sub>d\<^sub>d\<^sub>r) (Immediate w\<^sub>v\<^sub>a\<^sub>l\<^sub>_\<^sub>c\<^sub>o\<^sub>n\<^sub>c\<^sub>a\<^sub>t) (sz\<^sub>v\<^sub>a\<^sub>l - sz\<^sub>m\<^sub>e\<^sub>m) el)\<rbrakk> \<Longrightarrow> P mem w\<^sub>a\<^sub>d\<^sub>d\<^sub>r (Immediate w\<^sub>v\<^sub>a\<^sub>l) sz\<^sub>v\<^sub>a\<^sub>l el\<close>
+      and \<open>\<And>sz\<^sub>a\<^sub>d\<^sub>d\<^sub>r sz\<^sub>m\<^sub>e\<^sub>m str t. \<lbrakk>type mem = Mem sz\<^sub>a\<^sub>d\<^sub>d\<^sub>r sz\<^sub>m\<^sub>e\<^sub>m; sz\<^sub>m\<^sub>e\<^sub>m \<noteq> 0; sz\<^sub>v\<^sub>a\<^sub>l > sz\<^sub>m\<^sub>e\<^sub>m; v\<^sub>v\<^sub>a\<^sub>l = unknown[str]: t; v' = (
+            (store (mem[w\<^sub>a\<^sub>d\<^sub>d\<^sub>r \<leftarrow> (Unknown str (Imm sz\<^sub>m\<^sub>e\<^sub>m)), sz\<^sub>m\<^sub>e\<^sub>m]) (succ w\<^sub>a\<^sub>d\<^sub>d\<^sub>r) (unknown[str]: (Imm (sz\<^sub>v\<^sub>a\<^sub>l - sz\<^sub>m\<^sub>e\<^sub>m))) (sz\<^sub>v\<^sub>a\<^sub>l - sz\<^sub>m\<^sub>e\<^sub>m) en)
+        )\<rbrakk> \<Longrightarrow> P mem w\<^sub>a\<^sub>d\<^sub>d\<^sub>r v\<^sub>v\<^sub>a\<^sub>l sz\<^sub>v\<^sub>a\<^sub>l en\<close>
+      and \<open>\<And>sz\<^sub>a\<^sub>d\<^sub>d\<^sub>r sz\<^sub>m\<^sub>e\<^sub>m a b c d. \<lbrakk>type mem = Mem sz\<^sub>a\<^sub>d\<^sub>d\<^sub>r sz\<^sub>m\<^sub>e\<^sub>m; sz\<^sub>m\<^sub>e\<^sub>m \<noteq> 0; sz\<^sub>v\<^sub>a\<^sub>l > sz\<^sub>m\<^sub>e\<^sub>m; v\<^sub>v\<^sub>a\<^sub>l = (a[b \<leftarrow> c, d]); v' = undefined\<rbrakk> \<Longrightarrow> P mem w\<^sub>a\<^sub>d\<^sub>d\<^sub>r v\<^sub>v\<^sub>a\<^sub>l sz\<^sub>v\<^sub>a\<^sub>l en\<close>
+      and \<open>\<And>sz\<^sub>a\<^sub>d\<^sub>d\<^sub>r sz\<^sub>m\<^sub>e\<^sub>m. \<lbrakk>type mem = Mem sz\<^sub>a\<^sub>d\<^sub>d\<^sub>r sz\<^sub>m\<^sub>e\<^sub>m; sz\<^sub>m\<^sub>e\<^sub>m \<noteq> 0; sz\<^sub>m\<^sub>e\<^sub>m = sz\<^sub>v\<^sub>a\<^sub>l; v' = (mem[w\<^sub>a\<^sub>d\<^sub>d\<^sub>r \<leftarrow> v\<^sub>v\<^sub>a\<^sub>l, sz\<^sub>m\<^sub>e\<^sub>m])\<rbrakk> \<Longrightarrow> P mem w\<^sub>a\<^sub>d\<^sub>d\<^sub>r v\<^sub>v\<^sub>a\<^sub>l sz\<^sub>v\<^sub>a\<^sub>l en\<close>
+      and \<open>\<And>sz\<^sub>a\<^sub>d\<^sub>d\<^sub>r sz\<^sub>m\<^sub>e\<^sub>m. \<lbrakk>type mem = Mem sz\<^sub>a\<^sub>d\<^sub>d\<^sub>r sz\<^sub>m\<^sub>e\<^sub>m; sz\<^sub>m\<^sub>e\<^sub>m \<noteq> 0; sz\<^sub>m\<^sub>e\<^sub>m > sz\<^sub>v\<^sub>a\<^sub>l; v' = undefined\<rbrakk> \<Longrightarrow> P mem w\<^sub>a\<^sub>d\<^sub>d\<^sub>r v\<^sub>v\<^sub>a\<^sub>l sz\<^sub>v\<^sub>a\<^sub>l en\<close>
+      and \<open>\<And>sz\<^sub>a\<^sub>d\<^sub>d\<^sub>r sz\<^sub>m\<^sub>e\<^sub>m. \<lbrakk>type mem = Mem sz\<^sub>a\<^sub>d\<^sub>d\<^sub>r sz\<^sub>m\<^sub>e\<^sub>m; sz\<^sub>m\<^sub>e\<^sub>m = 0; v' = undefined\<rbrakk> \<Longrightarrow> P mem w\<^sub>a\<^sub>d\<^sub>d\<^sub>r v\<^sub>v\<^sub>a\<^sub>l sz\<^sub>v\<^sub>a\<^sub>l en\<close>
+      and \<open>\<And>sz. \<lbrakk>type mem = Imm sz; v' = undefined\<rbrakk> \<Longrightarrow> P mem w\<^sub>a\<^sub>d\<^sub>d\<^sub>r v\<^sub>v\<^sub>a\<^sub>l sz\<^sub>v\<^sub>a\<^sub>l en\<close>
+    shows \<open>P mem w\<^sub>a\<^sub>d\<^sub>d\<^sub>r v\<^sub>v\<^sub>a\<^sub>l sz\<^sub>v\<^sub>a\<^sub>l en\<close>
+  using assms(1) apply (cases \<open>type mem\<close>)
+  subgoal 
+    using assms(9) by auto
+  apply auto
+  apply (case_tac \<open>x22 = 0\<close>)
+  apply (simp add: assms(8))
+  apply (case_tac \<open>sz\<^sub>v\<^sub>a\<^sub>l < x22\<close>)
+  apply (simp add: assms(7))
+  apply (case_tac \<open>sz\<^sub>v\<^sub>a\<^sub>l > x22\<close>)
+  apply (auto simp del: store.simps)
+  defer
+  using assms(6) apply blast
+  apply (simp_all only: Let_def)
+  apply (cases v\<^sub>v\<^sub>a\<^sub>l)
+  apply (auto simp del: store.simps)
+  apply (cases en)
+  apply (auto simp del: store.simps extract_word.simps)
+  using assms(3) not_gr_zero diff_zero apply (metis extract_word.elims)
+  using assms(2) apply (metis less_numeral_extra(3))
+  using assms(4) apply blast
+  using assms(5) by blast
+
+thm store'.induct
+
+lemma store'_inducts[consumes 1]:
+  assumes \<open>v' = store' mem w\<^sub>a\<^sub>d\<^sub>d\<^sub>r v\<^sub>v\<^sub>a\<^sub>l sz\<^sub>v\<^sub>a\<^sub>l en\<close>
+      and \<open>(\<And>vstr sz\<^sub>a\<^sub>d\<^sub>d\<^sub>r sz\<^sub>m\<^sub>e\<^sub>m w\<^sub>a\<^sub>d\<^sub>d\<^sub>r w\<^sub>v\<^sub>a\<^sub>l sz\<^sub>v\<^sub>a\<^sub>l. bits w\<^sub>v\<^sub>a\<^sub>l = sz\<^sub>v\<^sub>a\<^sub>l \<Longrightarrow> sz\<^sub>m\<^sub>e\<^sub>m \<noteq> 0 \<Longrightarrow> sz\<^sub>m\<^sub>e\<^sub>m < sz\<^sub>v\<^sub>a\<^sub>l 
+             \<Longrightarrow> bits w\<^sub>a\<^sub>d\<^sub>d\<^sub>r = sz\<^sub>a\<^sub>d\<^sub>d\<^sub>r \<Longrightarrow>
+             P ((unknown[vstr]: Mem sz\<^sub>a\<^sub>d\<^sub>d\<^sub>r sz\<^sub>m\<^sub>e\<^sub>m)[w\<^sub>a\<^sub>d\<^sub>d\<^sub>r \<leftarrow> Immediate (ext w\<^sub>v\<^sub>a\<^sub>l \<sim> hi : sz\<^sub>m\<^sub>e\<^sub>m \<sim> lo : 0), sz\<^sub>m\<^sub>e\<^sub>m]) (succ w\<^sub>a\<^sub>d\<^sub>d\<^sub>r) (Immediate ext w\<^sub>v\<^sub>a\<^sub>l \<sim> hi : sz\<^sub>v\<^sub>a\<^sub>l \<sim> lo : sz\<^sub>m\<^sub>e\<^sub>m) (sz\<^sub>v\<^sub>a\<^sub>l - sz\<^sub>m\<^sub>e\<^sub>m) el
+            \<Longrightarrow> P (unknown[vstr]: (Mem sz\<^sub>a\<^sub>d\<^sub>d\<^sub>r sz\<^sub>m\<^sub>e\<^sub>m)) w\<^sub>a\<^sub>d\<^sub>d\<^sub>r (Immediate w\<^sub>v\<^sub>a\<^sub>l) sz\<^sub>v\<^sub>a\<^sub>l el)\<close>
+      and \<open>(\<And>vstr sz\<^sub>a\<^sub>d\<^sub>d\<^sub>r sz\<^sub>m\<^sub>e\<^sub>m w\<^sub>a\<^sub>d\<^sub>d\<^sub>r w\<^sub>v\<^sub>a\<^sub>l sz\<^sub>v\<^sub>a\<^sub>l. bits w\<^sub>v\<^sub>a\<^sub>l = sz\<^sub>v\<^sub>a\<^sub>l \<Longrightarrow> sz\<^sub>m\<^sub>e\<^sub>m \<noteq> 0 \<Longrightarrow> sz\<^sub>m\<^sub>e\<^sub>m < sz\<^sub>v\<^sub>a\<^sub>l 
+             \<Longrightarrow> bits w\<^sub>a\<^sub>d\<^sub>d\<^sub>r = sz\<^sub>a\<^sub>d\<^sub>d\<^sub>r \<Longrightarrow>
+             P (unknown[vstr]: Mem sz\<^sub>a\<^sub>d\<^sub>d\<^sub>r sz\<^sub>m\<^sub>e\<^sub>m)[w\<^sub>a\<^sub>d\<^sub>d\<^sub>r \<leftarrow> Immediate (ext w\<^sub>v\<^sub>a\<^sub>l \<sim> hi : sz\<^sub>v\<^sub>a\<^sub>l \<sim> lo : sz\<^sub>v\<^sub>a\<^sub>l - sz\<^sub>m\<^sub>e\<^sub>m), sz\<^sub>m\<^sub>e\<^sub>m] (succ w\<^sub>a\<^sub>d\<^sub>d\<^sub>r) (Immediate ext w\<^sub>v\<^sub>a\<^sub>l \<sim> hi : sz\<^sub>v\<^sub>a\<^sub>l - sz\<^sub>m\<^sub>e\<^sub>m \<sim> lo : 0) (sz\<^sub>v\<^sub>a\<^sub>l - sz\<^sub>m\<^sub>e\<^sub>m) be
+            \<Longrightarrow> P (unknown[vstr]: (Mem sz\<^sub>a\<^sub>d\<^sub>d\<^sub>r sz\<^sub>m\<^sub>e\<^sub>m)) w\<^sub>a\<^sub>d\<^sub>d\<^sub>r (Immediate w\<^sub>v\<^sub>a\<^sub>l) sz\<^sub>v\<^sub>a\<^sub>l be)\<close>
+      and \<open>(\<And>vstr sz\<^sub>a\<^sub>d\<^sub>d\<^sub>r sz\<^sub>m\<^sub>e\<^sub>m w\<^sub>a\<^sub>d\<^sub>d\<^sub>r str sz sz\<^sub>v\<^sub>a\<^sub>l en. sz = sz\<^sub>v\<^sub>a\<^sub>l \<Longrightarrow> sz\<^sub>m\<^sub>e\<^sub>m \<noteq> 0 \<Longrightarrow> sz\<^sub>m\<^sub>e\<^sub>m < sz\<^sub>v\<^sub>a\<^sub>l 
+             \<Longrightarrow> bits w\<^sub>a\<^sub>d\<^sub>d\<^sub>r = sz\<^sub>a\<^sub>d\<^sub>d\<^sub>r \<Longrightarrow>
+             P ((unknown[vstr]: Mem sz\<^sub>a\<^sub>d\<^sub>d\<^sub>r sz\<^sub>m\<^sub>e\<^sub>m)[w\<^sub>a\<^sub>d\<^sub>d\<^sub>r \<leftarrow> (unknown[str]: Imm sz\<^sub>m\<^sub>e\<^sub>m), sz\<^sub>m\<^sub>e\<^sub>m]) (succ w\<^sub>a\<^sub>d\<^sub>d\<^sub>r) unknown[str]: Imm (sz\<^sub>v\<^sub>a\<^sub>l - sz\<^sub>m\<^sub>e\<^sub>m) (sz\<^sub>v\<^sub>a\<^sub>l - sz\<^sub>m\<^sub>e\<^sub>m) en
+            \<Longrightarrow> P (unknown[vstr]: (Mem sz\<^sub>a\<^sub>d\<^sub>d\<^sub>r sz\<^sub>m\<^sub>e\<^sub>m)) w\<^sub>a\<^sub>d\<^sub>d\<^sub>r (unknown[str]: (Imm sz)) sz\<^sub>v\<^sub>a\<^sub>l en) \<close>
+
+      and \<open>(\<And>memR wR vR sz\<^sub>m\<^sub>e\<^sub>m w\<^sub>a\<^sub>d\<^sub>d\<^sub>r w\<^sub>v\<^sub>a\<^sub>l sz\<^sub>v\<^sub>a\<^sub>l. bits w\<^sub>v\<^sub>a\<^sub>l = sz\<^sub>v\<^sub>a\<^sub>l \<Longrightarrow> sz\<^sub>m\<^sub>e\<^sub>m \<noteq> 0 \<Longrightarrow> sz\<^sub>m\<^sub>e\<^sub>m < sz\<^sub>v\<^sub>a\<^sub>l 
+             \<Longrightarrow> bits w\<^sub>a\<^sub>d\<^sub>d\<^sub>r = bits wR \<Longrightarrow> 
+             P memR[wR \<leftarrow> vR, sz\<^sub>m\<^sub>e\<^sub>m][w\<^sub>a\<^sub>d\<^sub>d\<^sub>r \<leftarrow> Immediate( ext w\<^sub>v\<^sub>a\<^sub>l \<sim> hi : sz\<^sub>v\<^sub>a\<^sub>l \<sim> lo : (sz\<^sub>v\<^sub>a\<^sub>l - sz\<^sub>m\<^sub>e\<^sub>m)), sz\<^sub>m\<^sub>e\<^sub>m] (succ w\<^sub>a\<^sub>d\<^sub>d\<^sub>r) (Immediate ext w\<^sub>v\<^sub>a\<^sub>l \<sim> hi : sz\<^sub>v\<^sub>a\<^sub>l - sz\<^sub>m\<^sub>e\<^sub>m \<sim> lo : 0) (sz\<^sub>v\<^sub>a\<^sub>l - sz\<^sub>m\<^sub>e\<^sub>m) be
+            \<Longrightarrow> P memR[wR \<leftarrow> vR, sz\<^sub>m\<^sub>e\<^sub>m] w\<^sub>a\<^sub>d\<^sub>d\<^sub>r (Immediate w\<^sub>v\<^sub>a\<^sub>l) sz\<^sub>v\<^sub>a\<^sub>l be)\<close>
+      and \<open>(\<And>memR wR vR sz\<^sub>m\<^sub>e\<^sub>m w\<^sub>a\<^sub>d\<^sub>d\<^sub>r w\<^sub>v\<^sub>a\<^sub>l sz\<^sub>v\<^sub>a\<^sub>l. bits w\<^sub>v\<^sub>a\<^sub>l = sz\<^sub>v\<^sub>a\<^sub>l \<Longrightarrow> sz\<^sub>m\<^sub>e\<^sub>m \<noteq> 0 \<Longrightarrow> sz\<^sub>m\<^sub>e\<^sub>m < sz\<^sub>v\<^sub>a\<^sub>l 
+             \<Longrightarrow> bits w\<^sub>a\<^sub>d\<^sub>d\<^sub>r = bits wR \<Longrightarrow> (
+            P memR[wR \<leftarrow> vR, sz\<^sub>m\<^sub>e\<^sub>m][w\<^sub>a\<^sub>d\<^sub>d\<^sub>r \<leftarrow> Immediate (ext w\<^sub>v\<^sub>a\<^sub>l \<sim> hi : sz\<^sub>m\<^sub>e\<^sub>m \<sim> lo : 0), sz\<^sub>m\<^sub>e\<^sub>m] (succ w\<^sub>a\<^sub>d\<^sub>d\<^sub>r) (Immediate ext w\<^sub>v\<^sub>a\<^sub>l \<sim> hi : sz\<^sub>v\<^sub>a\<^sub>l \<sim> lo : sz\<^sub>m\<^sub>e\<^sub>m) (sz\<^sub>v\<^sub>a\<^sub>l - sz\<^sub>m\<^sub>e\<^sub>m) el) 
+            \<Longrightarrow> P memR[wR \<leftarrow> vR, sz\<^sub>m\<^sub>e\<^sub>m] w\<^sub>a\<^sub>d\<^sub>d\<^sub>r (Immediate w\<^sub>v\<^sub>a\<^sub>l) sz\<^sub>v\<^sub>a\<^sub>l el) \<close>
+      and \<open>(\<And>memR wR vR sz\<^sub>m\<^sub>e\<^sub>m w\<^sub>a\<^sub>d\<^sub>d\<^sub>r str sz sz\<^sub>v\<^sub>a\<^sub>l en. sz = sz\<^sub>v\<^sub>a\<^sub>l \<Longrightarrow> sz\<^sub>m\<^sub>e\<^sub>m \<noteq> 0 \<Longrightarrow> sz\<^sub>m\<^sub>e\<^sub>m < sz\<^sub>v\<^sub>a\<^sub>l 
+             \<Longrightarrow> bits w\<^sub>a\<^sub>d\<^sub>d\<^sub>r = bits wR \<Longrightarrow>
+            P (memR[wR \<leftarrow> vR, sz\<^sub>m\<^sub>e\<^sub>m][w\<^sub>a\<^sub>d\<^sub>d\<^sub>r \<leftarrow> (unknown[str]: Imm sz\<^sub>m\<^sub>e\<^sub>m), sz\<^sub>m\<^sub>e\<^sub>m]) (succ w\<^sub>a\<^sub>d\<^sub>d\<^sub>r) (unknown[str]: Imm (sz\<^sub>v\<^sub>a\<^sub>l - sz\<^sub>m\<^sub>e\<^sub>m)) (sz\<^sub>v\<^sub>a\<^sub>l - sz\<^sub>m\<^sub>e\<^sub>m) en 
+            \<Longrightarrow> P (memR[wR \<leftarrow> vR, sz\<^sub>m\<^sub>e\<^sub>m]) w\<^sub>a\<^sub>d\<^sub>d\<^sub>r (unknown[str]: (Imm sz)) sz\<^sub>v\<^sub>a\<^sub>l en)\<close>
+
+      and \<open>(\<And>vstr sz\<^sub>a\<^sub>d\<^sub>d\<^sub>r sz\<^sub>m\<^sub>e\<^sub>m w\<^sub>a\<^sub>d\<^sub>d\<^sub>r str w\<^sub>v\<^sub>a\<^sub>l sz\<^sub>v\<^sub>a\<^sub>l en. bits w\<^sub>v\<^sub>a\<^sub>l = sz\<^sub>v\<^sub>a\<^sub>l \<Longrightarrow> sz\<^sub>v\<^sub>a\<^sub>l = sz\<^sub>m\<^sub>e\<^sub>m \<Longrightarrow> sz\<^sub>m\<^sub>e\<^sub>m > 0 \<Longrightarrow> bits w\<^sub>a\<^sub>d\<^sub>d\<^sub>r = sz\<^sub>a\<^sub>d\<^sub>d\<^sub>r
+            \<Longrightarrow> P (unknown[vstr]: (Mem sz\<^sub>a\<^sub>d\<^sub>d\<^sub>r sz\<^sub>m\<^sub>e\<^sub>m)) w\<^sub>a\<^sub>d\<^sub>d\<^sub>r (Immediate w\<^sub>v\<^sub>a\<^sub>l) sz\<^sub>v\<^sub>a\<^sub>l en)\<close>
+      and \<open>(\<And>vstr sz\<^sub>a\<^sub>d\<^sub>d\<^sub>r sz\<^sub>m\<^sub>e\<^sub>m w\<^sub>a\<^sub>d\<^sub>d\<^sub>r str sz sz\<^sub>v\<^sub>a\<^sub>l en. sz = sz\<^sub>v\<^sub>a\<^sub>l \<Longrightarrow> sz\<^sub>v\<^sub>a\<^sub>l = sz\<^sub>m\<^sub>e\<^sub>m \<Longrightarrow> sz\<^sub>m\<^sub>e\<^sub>m > 0 \<Longrightarrow> bits w\<^sub>a\<^sub>d\<^sub>d\<^sub>r = sz\<^sub>a\<^sub>d\<^sub>d\<^sub>r
+            \<Longrightarrow> P (unknown[vstr]: (Mem sz\<^sub>a\<^sub>d\<^sub>d\<^sub>r sz\<^sub>m\<^sub>e\<^sub>m)) w\<^sub>a\<^sub>d\<^sub>d\<^sub>r (unknown[str]: (Imm sz)) sz\<^sub>v\<^sub>a\<^sub>l en)\<close>
+
+      and \<open>(\<And>memR wR vR sz\<^sub>m\<^sub>e\<^sub>m w\<^sub>a\<^sub>d\<^sub>d\<^sub>r str w\<^sub>v\<^sub>a\<^sub>l sz\<^sub>v\<^sub>a\<^sub>l en. bits w\<^sub>v\<^sub>a\<^sub>l = sz\<^sub>v\<^sub>a\<^sub>l \<Longrightarrow> sz\<^sub>v\<^sub>a\<^sub>l = sz\<^sub>m\<^sub>e\<^sub>m \<Longrightarrow> sz\<^sub>m\<^sub>e\<^sub>m > 0
+            \<Longrightarrow> bits w\<^sub>a\<^sub>d\<^sub>d\<^sub>r = bits wR \<Longrightarrow> P (memR[wR \<leftarrow> vR, sz\<^sub>m\<^sub>e\<^sub>m]) w\<^sub>a\<^sub>d\<^sub>d\<^sub>r (Immediate w\<^sub>v\<^sub>a\<^sub>l) sz\<^sub>v\<^sub>a\<^sub>l en)\<close>
+      and \<open>(\<And>memR wR vR sz\<^sub>m\<^sub>e\<^sub>m w\<^sub>a\<^sub>d\<^sub>d\<^sub>r str sz sz\<^sub>v\<^sub>a\<^sub>l en. sz = sz\<^sub>v\<^sub>a\<^sub>l \<Longrightarrow> sz\<^sub>v\<^sub>a\<^sub>l = sz\<^sub>m\<^sub>e\<^sub>m \<Longrightarrow> sz\<^sub>m\<^sub>e\<^sub>m > 0
+            \<Longrightarrow> bits w\<^sub>a\<^sub>d\<^sub>d\<^sub>r = bits wR \<Longrightarrow> P (memR[wR \<leftarrow> vR, sz\<^sub>m\<^sub>e\<^sub>m]) w\<^sub>a\<^sub>d\<^sub>d\<^sub>r (unknown[str]: (Imm sz)) sz\<^sub>v\<^sub>a\<^sub>l en)\<close>
+
+      (* Invalid cases *)
+      and \<open>(\<And>vstr sz\<^sub>a\<^sub>d\<^sub>d\<^sub>r sz\<^sub>m\<^sub>e\<^sub>m w\<^sub>a\<^sub>d\<^sub>d\<^sub>r str v\<^sub>v\<^sub>a\<^sub>l sz\<^sub>v\<^sub>a\<^sub>l en. bits w\<^sub>a\<^sub>d\<^sub>d\<^sub>r \<noteq> sz\<^sub>a\<^sub>d\<^sub>d\<^sub>r
+            \<Longrightarrow> P (unknown[vstr]: (Mem sz\<^sub>a\<^sub>d\<^sub>d\<^sub>r sz\<^sub>m\<^sub>e\<^sub>m)) w\<^sub>a\<^sub>d\<^sub>d\<^sub>r v\<^sub>v\<^sub>a\<^sub>l sz\<^sub>v\<^sub>a\<^sub>l en)\<close>
+      and \<open>(\<And>memR wR vR sz\<^sub>m\<^sub>e\<^sub>m w\<^sub>a\<^sub>d\<^sub>d\<^sub>r str v\<^sub>v\<^sub>a\<^sub>l sz\<^sub>v\<^sub>a\<^sub>l en. bits w\<^sub>a\<^sub>d\<^sub>d\<^sub>r \<noteq> bits wR
+            \<Longrightarrow> P (memR[wR \<leftarrow> vR, sz\<^sub>m\<^sub>e\<^sub>m]) w\<^sub>a\<^sub>d\<^sub>d\<^sub>r v\<^sub>v\<^sub>a\<^sub>l sz\<^sub>v\<^sub>a\<^sub>l en)\<close>
+      and \<open>(\<And>vstr sz\<^sub>a\<^sub>d\<^sub>d\<^sub>r sz\<^sub>m\<^sub>e\<^sub>m w\<^sub>a\<^sub>d\<^sub>d\<^sub>r str v\<^sub>v\<^sub>a\<^sub>l sz\<^sub>v\<^sub>a\<^sub>l en. sz\<^sub>v\<^sub>a\<^sub>l < sz\<^sub>m\<^sub>e\<^sub>m
+            \<Longrightarrow> P (unknown[vstr]: (Mem sz\<^sub>a\<^sub>d\<^sub>d\<^sub>r sz\<^sub>m\<^sub>e\<^sub>m)) w\<^sub>a\<^sub>d\<^sub>d\<^sub>r v\<^sub>v\<^sub>a\<^sub>l sz\<^sub>v\<^sub>a\<^sub>l en)\<close>
+      and \<open>(\<And>memR wR vR sz\<^sub>m\<^sub>e\<^sub>m w\<^sub>a\<^sub>d\<^sub>d\<^sub>r str v\<^sub>v\<^sub>a\<^sub>l sz\<^sub>v\<^sub>a\<^sub>l en. sz\<^sub>v\<^sub>a\<^sub>l < sz\<^sub>m\<^sub>e\<^sub>m
+            \<Longrightarrow> P (memR[wR \<leftarrow> vR, sz\<^sub>m\<^sub>e\<^sub>m]) w\<^sub>a\<^sub>d\<^sub>d\<^sub>r v\<^sub>v\<^sub>a\<^sub>l sz\<^sub>v\<^sub>a\<^sub>l en)\<close>
+      and \<open>(\<And>vstr sz\<^sub>a\<^sub>d\<^sub>d\<^sub>r sz\<^sub>m\<^sub>e\<^sub>m w\<^sub>a\<^sub>d\<^sub>d\<^sub>r str v\<^sub>v\<^sub>a\<^sub>l sz\<^sub>v\<^sub>a\<^sub>l en. sz\<^sub>m\<^sub>e\<^sub>m = 0
+            \<Longrightarrow> P (unknown[vstr]: (Mem sz\<^sub>a\<^sub>d\<^sub>d\<^sub>r sz\<^sub>m\<^sub>e\<^sub>m)) w\<^sub>a\<^sub>d\<^sub>d\<^sub>r v\<^sub>v\<^sub>a\<^sub>l sz\<^sub>v\<^sub>a\<^sub>l en)\<close>
+      and \<open>(\<And>memR wR vR sz\<^sub>m\<^sub>e\<^sub>m w\<^sub>a\<^sub>d\<^sub>d\<^sub>r str v\<^sub>v\<^sub>a\<^sub>l sz\<^sub>v\<^sub>a\<^sub>l en. sz\<^sub>m\<^sub>e\<^sub>m = 0
+            \<Longrightarrow> P (memR[wR \<leftarrow> vR, sz\<^sub>m\<^sub>e\<^sub>m]) w\<^sub>a\<^sub>d\<^sub>d\<^sub>r v\<^sub>v\<^sub>a\<^sub>l sz\<^sub>v\<^sub>a\<^sub>l en)\<close>
+      and \<open>(\<And>mem w\<^sub>a\<^sub>d\<^sub>d\<^sub>r str sz sz\<^sub>v\<^sub>a\<^sub>l en. sz \<noteq> sz\<^sub>v\<^sub>a\<^sub>l
+            \<Longrightarrow> P mem w\<^sub>a\<^sub>d\<^sub>d\<^sub>r (unknown[str]: (Imm sz)) sz\<^sub>v\<^sub>a\<^sub>l en)\<close>
+      and \<open>(\<And>mem w\<^sub>a\<^sub>d\<^sub>d\<^sub>r str w\<^sub>v\<^sub>a\<^sub>l sz\<^sub>v\<^sub>a\<^sub>l en. bits w\<^sub>v\<^sub>a\<^sub>l \<noteq> sz\<^sub>v\<^sub>a\<^sub>l
+            \<Longrightarrow> P mem w\<^sub>a\<^sub>d\<^sub>d\<^sub>r (Immediate w\<^sub>v\<^sub>a\<^sub>l) sz\<^sub>v\<^sub>a\<^sub>l en)\<close>
+      and \<open>(\<And>v uv uw ux uy. P (Immediate v) uv uw ux uy)\<close>
+      and \<open>(\<And>v vb uv uw ux uy. P (unknown[v]: (Imm vb)) uv uw ux uy)\<close>
+      and \<open>(\<And>uu uv v va vb vc ux uy. P uu uv (v[va \<leftarrow> vb, vc]) ux uy)\<close>
+      and \<open>(\<And>uu uv v vf vg vd ux uy. P uu uv (unknown[vd]: (Mem vf vg)) ux uy)\<close>
+    shows \<open>P mem w\<^sub>a\<^sub>d\<^sub>d\<^sub>r v\<^sub>v\<^sub>a\<^sub>l sz\<^sub>v\<^sub>a\<^sub>l en\<close>
+  using assms(1) gr0I apply (induct rule: store'.induct)
+  using assms(8-23) apply (auto simp del: store'.simps extract_word.simps)
+  using assms(2) store'.simps(1) apply (metis not_less_iff_gr_or_eq)
+  using assms(3) store'.simps(2) apply (metis not_less_iff_gr_or_eq)
+  using assms(4) store'.simps(3) apply (metis not_less_iff_gr_or_eq)
+  using assms(5) store'.simps(4) apply (metis (no_types, lifting) not_less_iff_gr_or_eq)
+  using assms(6) store'.simps(5) apply (metis (no_types, lifting) not_less_iff_gr_or_eq)
+  using assms(7) store'.simps(6) by (metis not_less_iff_gr_or_eq)
+
+
+lemma store''_inducts[consumes 1]:
+  assumes \<open>v' = store' mem w\<^sub>a\<^sub>d\<^sub>d\<^sub>r v\<^sub>v\<^sub>a\<^sub>l sz\<^sub>v\<^sub>a\<^sub>l en\<close>
+      and \<open>(\<And>mem sz\<^sub>a\<^sub>d\<^sub>d\<^sub>r sz\<^sub>m\<^sub>e\<^sub>m w\<^sub>a\<^sub>d\<^sub>d\<^sub>r w\<^sub>v\<^sub>a\<^sub>l sz\<^sub>v\<^sub>a\<^sub>l. \<lbrakk>type mem = Mem sz\<^sub>a\<^sub>d\<^sub>d\<^sub>r sz\<^sub>m\<^sub>e\<^sub>m; bits w\<^sub>v\<^sub>a\<^sub>l = sz\<^sub>v\<^sub>a\<^sub>l; sz\<^sub>m\<^sub>e\<^sub>m \<noteq> 0; sz\<^sub>m\<^sub>e\<^sub>m < sz\<^sub>v\<^sub>a\<^sub>l;
+             bits w\<^sub>a\<^sub>d\<^sub>d\<^sub>r = sz\<^sub>a\<^sub>d\<^sub>d\<^sub>r;
+             P mem[w\<^sub>a\<^sub>d\<^sub>d\<^sub>r \<leftarrow> Immediate ext w\<^sub>v\<^sub>a\<^sub>l \<sim> hi : sz\<^sub>v\<^sub>a\<^sub>l \<sim> lo : sz\<^sub>v\<^sub>a\<^sub>l - sz\<^sub>m\<^sub>e\<^sub>m, sz\<^sub>m\<^sub>e\<^sub>m] (succ w\<^sub>a\<^sub>d\<^sub>d\<^sub>r) (Immediate ext w\<^sub>v\<^sub>a\<^sub>l \<sim> hi : sz\<^sub>v\<^sub>a\<^sub>l - sz\<^sub>m\<^sub>e\<^sub>m \<sim> lo : 0) (sz\<^sub>v\<^sub>a\<^sub>l - sz\<^sub>m\<^sub>e\<^sub>m) be\<rbrakk>
+            \<Longrightarrow> P mem w\<^sub>a\<^sub>d\<^sub>d\<^sub>r (Immediate w\<^sub>v\<^sub>a\<^sub>l) sz\<^sub>v\<^sub>a\<^sub>l be)\<close>
+
+      and \<open>(\<And>mem sz\<^sub>a\<^sub>d\<^sub>d\<^sub>r sz\<^sub>m\<^sub>e\<^sub>m w\<^sub>a\<^sub>d\<^sub>d\<^sub>r w\<^sub>v\<^sub>a\<^sub>l sz\<^sub>v\<^sub>a\<^sub>l. \<lbrakk>type mem = Mem sz\<^sub>a\<^sub>d\<^sub>d\<^sub>r sz\<^sub>m\<^sub>e\<^sub>m; bits w\<^sub>v\<^sub>a\<^sub>l = sz\<^sub>v\<^sub>a\<^sub>l; sz\<^sub>m\<^sub>e\<^sub>m \<noteq> 0; sz\<^sub>m\<^sub>e\<^sub>m < sz\<^sub>v\<^sub>a\<^sub>l;
+             bits w\<^sub>a\<^sub>d\<^sub>d\<^sub>r = sz\<^sub>a\<^sub>d\<^sub>d\<^sub>r;
+             P mem[w\<^sub>a\<^sub>d\<^sub>d\<^sub>r \<leftarrow> Immediate ext w\<^sub>v\<^sub>a\<^sub>l \<sim> hi : sz\<^sub>m\<^sub>e\<^sub>m \<sim> lo : 0, sz\<^sub>m\<^sub>e\<^sub>m] (succ w\<^sub>a\<^sub>d\<^sub>d\<^sub>r) (Immediate ext w\<^sub>v\<^sub>a\<^sub>l \<sim> hi : sz\<^sub>v\<^sub>a\<^sub>l \<sim> lo : sz\<^sub>m\<^sub>e\<^sub>m) (sz\<^sub>v\<^sub>a\<^sub>l - sz\<^sub>m\<^sub>e\<^sub>m) el\<rbrakk>
+            \<Longrightarrow> P mem w\<^sub>a\<^sub>d\<^sub>d\<^sub>r (Immediate w\<^sub>v\<^sub>a\<^sub>l) sz\<^sub>v\<^sub>a\<^sub>l el) \<close>
+
+      and \<open>(\<And>mem sz\<^sub>a\<^sub>d\<^sub>d\<^sub>r sz\<^sub>m\<^sub>e\<^sub>m w\<^sub>a\<^sub>d\<^sub>d\<^sub>r str sz sz\<^sub>v\<^sub>a\<^sub>l en. \<lbrakk>type mem = Mem sz\<^sub>a\<^sub>d\<^sub>d\<^sub>r sz\<^sub>m\<^sub>e\<^sub>m; sz = sz\<^sub>v\<^sub>a\<^sub>l; sz\<^sub>m\<^sub>e\<^sub>m \<noteq> 0; sz\<^sub>m\<^sub>e\<^sub>m < sz\<^sub>v\<^sub>a\<^sub>l;
+             bits w\<^sub>a\<^sub>d\<^sub>d\<^sub>r = sz\<^sub>a\<^sub>d\<^sub>d\<^sub>r;
+             P mem[w\<^sub>a\<^sub>d\<^sub>d\<^sub>r \<leftarrow> (unknown[str]: Imm sz\<^sub>m\<^sub>e\<^sub>m), sz\<^sub>m\<^sub>e\<^sub>m] (succ w\<^sub>a\<^sub>d\<^sub>d\<^sub>r) (unknown[str]: Imm (sz\<^sub>v\<^sub>a\<^sub>l - sz\<^sub>m\<^sub>e\<^sub>m)) (sz\<^sub>v\<^sub>a\<^sub>l - sz\<^sub>m\<^sub>e\<^sub>m) en\<rbrakk>
+            \<Longrightarrow> P mem w\<^sub>a\<^sub>d\<^sub>d\<^sub>r (unknown[str]: (Imm sz)) sz\<^sub>v\<^sub>a\<^sub>l en) \<close>
+
+      and \<open>(\<And>mem sz\<^sub>a\<^sub>d\<^sub>d\<^sub>r sz\<^sub>m\<^sub>e\<^sub>m w\<^sub>a\<^sub>d\<^sub>d\<^sub>r sz v\<^sub>v\<^sub>a\<^sub>l sz\<^sub>v\<^sub>a\<^sub>l en. \<lbrakk>type mem = Mem sz\<^sub>a\<^sub>d\<^sub>d\<^sub>r sz\<^sub>m\<^sub>e\<^sub>m; type v\<^sub>v\<^sub>a\<^sub>l = Imm sz; sz = sz\<^sub>v\<^sub>a\<^sub>l; sz\<^sub>v\<^sub>a\<^sub>l = sz\<^sub>m\<^sub>e\<^sub>m; sz\<^sub>m\<^sub>e\<^sub>m > 0; bits w\<^sub>a\<^sub>d\<^sub>d\<^sub>r = sz\<^sub>a\<^sub>d\<^sub>d\<^sub>r\<rbrakk>
+            \<Longrightarrow> P mem w\<^sub>a\<^sub>d\<^sub>d\<^sub>r v\<^sub>v\<^sub>a\<^sub>l sz\<^sub>v\<^sub>a\<^sub>l en)\<close>
+
+      (* Invalid cases *)
+      and \<open>(\<And>mem sz\<^sub>a\<^sub>d\<^sub>d\<^sub>r sz\<^sub>m\<^sub>e\<^sub>m w\<^sub>a\<^sub>d\<^sub>d\<^sub>r v\<^sub>v\<^sub>a\<^sub>l sz\<^sub>v\<^sub>a\<^sub>l en. \<lbrakk>type mem = Mem sz\<^sub>a\<^sub>d\<^sub>d\<^sub>r sz\<^sub>m\<^sub>e\<^sub>m; bits w\<^sub>a\<^sub>d\<^sub>d\<^sub>r \<noteq> sz\<^sub>a\<^sub>d\<^sub>d\<^sub>r\<rbrakk>
+            \<Longrightarrow> P mem w\<^sub>a\<^sub>d\<^sub>d\<^sub>r v\<^sub>v\<^sub>a\<^sub>l sz\<^sub>v\<^sub>a\<^sub>l en)\<close>
+      and \<open>(\<And>mem sz\<^sub>a\<^sub>d\<^sub>d\<^sub>r sz\<^sub>m\<^sub>e\<^sub>m w\<^sub>a\<^sub>d\<^sub>d\<^sub>r v\<^sub>v\<^sub>a\<^sub>l sz\<^sub>v\<^sub>a\<^sub>l en. \<lbrakk>type mem = Mem sz\<^sub>a\<^sub>d\<^sub>d\<^sub>r sz\<^sub>m\<^sub>e\<^sub>m; sz\<^sub>v\<^sub>a\<^sub>l < sz\<^sub>m\<^sub>e\<^sub>m\<rbrakk>
+            \<Longrightarrow> P mem w\<^sub>a\<^sub>d\<^sub>d\<^sub>r v\<^sub>v\<^sub>a\<^sub>l sz\<^sub>v\<^sub>a\<^sub>l en)\<close>
+      and \<open>(\<And>mem sz\<^sub>a\<^sub>d\<^sub>d\<^sub>r sz\<^sub>m\<^sub>e\<^sub>m w\<^sub>a\<^sub>d\<^sub>d\<^sub>r v\<^sub>v\<^sub>a\<^sub>l sz\<^sub>v\<^sub>a\<^sub>l en. \<lbrakk>type mem = Mem sz\<^sub>a\<^sub>d\<^sub>d\<^sub>r sz\<^sub>m\<^sub>e\<^sub>m; sz\<^sub>m\<^sub>e\<^sub>m = 0\<rbrakk>
+            \<Longrightarrow> P mem w\<^sub>a\<^sub>d\<^sub>d\<^sub>r v\<^sub>v\<^sub>a\<^sub>l sz\<^sub>v\<^sub>a\<^sub>l en)\<close>
+      and \<open>(\<And>mem w\<^sub>a\<^sub>d\<^sub>d\<^sub>r v\<^sub>v\<^sub>a\<^sub>l sz sz\<^sub>v\<^sub>a\<^sub>l en. \<lbrakk>type v\<^sub>v\<^sub>a\<^sub>l = Imm sz; sz \<noteq> sz\<^sub>v\<^sub>a\<^sub>l\<rbrakk>
+            \<Longrightarrow> P mem w\<^sub>a\<^sub>d\<^sub>d\<^sub>r v\<^sub>v\<^sub>a\<^sub>l sz\<^sub>v\<^sub>a\<^sub>l en)\<close>
+      and \<open>(\<And>mem sz uv uw ux uy. type mem = Imm sz \<Longrightarrow> P mem uv uw ux uy)\<close>
+      and \<open>(\<And>uu uv v\<^sub>v\<^sub>a\<^sub>l sz\<^sub>a\<^sub>d\<^sub>d\<^sub>r sz\<^sub>m\<^sub>e\<^sub>m ux uy. type v\<^sub>v\<^sub>a\<^sub>l = Mem sz\<^sub>a\<^sub>d\<^sub>d\<^sub>r sz\<^sub>m\<^sub>e\<^sub>m \<Longrightarrow> P uu uv v\<^sub>v\<^sub>a\<^sub>l ux uy)\<close>
+    shows \<open>P mem w\<^sub>a\<^sub>d\<^sub>d\<^sub>r v\<^sub>v\<^sub>a\<^sub>l sz\<^sub>v\<^sub>a\<^sub>l en\<close>
+  using assms type.simps apply (erule_tac store'_inducts)
+  by metis+
+
+lemma store'''_inducts[consumes 1]:
+  assumes \<open>v' = store' mem w\<^sub>a\<^sub>d\<^sub>d\<^sub>r v\<^sub>v\<^sub>a\<^sub>l sz\<^sub>v\<^sub>a\<^sub>l en\<close>
+      and \<open>(\<And>mem sz\<^sub>a\<^sub>d\<^sub>d\<^sub>r sz\<^sub>m\<^sub>e\<^sub>m w\<^sub>a\<^sub>d\<^sub>d\<^sub>r w\<^sub>v\<^sub>a\<^sub>l sz\<^sub>v\<^sub>a\<^sub>l. \<lbrakk>type mem = Mem sz\<^sub>a\<^sub>d\<^sub>d\<^sub>r sz\<^sub>m\<^sub>e\<^sub>m; bits w\<^sub>v\<^sub>a\<^sub>l = sz\<^sub>v\<^sub>a\<^sub>l; sz\<^sub>m\<^sub>e\<^sub>m \<noteq> 0; sz\<^sub>m\<^sub>e\<^sub>m < sz\<^sub>v\<^sub>a\<^sub>l;
+             bits w\<^sub>a\<^sub>d\<^sub>d\<^sub>r = sz\<^sub>a\<^sub>d\<^sub>d\<^sub>r;
+             P mem[w\<^sub>a\<^sub>d\<^sub>d\<^sub>r \<leftarrow> Immediate (ext w\<^sub>v\<^sub>a\<^sub>l \<sim> hi : sz\<^sub>v\<^sub>a\<^sub>l \<sim> lo : (sz\<^sub>v\<^sub>a\<^sub>l - sz\<^sub>m\<^sub>e\<^sub>m)), sz\<^sub>m\<^sub>e\<^sub>m] (succ w\<^sub>a\<^sub>d\<^sub>d\<^sub>r) (Immediate (ext w\<^sub>v\<^sub>a\<^sub>l \<sim> hi : (sz\<^sub>v\<^sub>a\<^sub>l - sz\<^sub>m\<^sub>e\<^sub>m) \<sim> lo : 0)) (sz\<^sub>v\<^sub>a\<^sub>l - sz\<^sub>m\<^sub>e\<^sub>m) be\<rbrakk>
+            \<Longrightarrow> P mem w\<^sub>a\<^sub>d\<^sub>d\<^sub>r (Immediate w\<^sub>v\<^sub>a\<^sub>l) sz\<^sub>v\<^sub>a\<^sub>l be)\<close>
+
+      and \<open>(\<And>mem sz\<^sub>a\<^sub>d\<^sub>d\<^sub>r sz\<^sub>m\<^sub>e\<^sub>m w\<^sub>a\<^sub>d\<^sub>d\<^sub>r w\<^sub>v\<^sub>a\<^sub>l sz\<^sub>v\<^sub>a\<^sub>l. \<lbrakk>type mem = Mem sz\<^sub>a\<^sub>d\<^sub>d\<^sub>r sz\<^sub>m\<^sub>e\<^sub>m; bits w\<^sub>v\<^sub>a\<^sub>l = sz\<^sub>v\<^sub>a\<^sub>l; sz\<^sub>m\<^sub>e\<^sub>m \<noteq> 0; sz\<^sub>m\<^sub>e\<^sub>m < sz\<^sub>v\<^sub>a\<^sub>l;
+             bits w\<^sub>a\<^sub>d\<^sub>d\<^sub>r = sz\<^sub>a\<^sub>d\<^sub>d\<^sub>r;
+             P mem[w\<^sub>a\<^sub>d\<^sub>d\<^sub>r \<leftarrow> Immediate (ext w\<^sub>v\<^sub>a\<^sub>l \<sim> hi : sz\<^sub>m\<^sub>e\<^sub>m \<sim> lo : 0), sz\<^sub>m\<^sub>e\<^sub>m] (succ w\<^sub>a\<^sub>d\<^sub>d\<^sub>r) (Immediate ext w\<^sub>v\<^sub>a\<^sub>l \<sim> hi : sz\<^sub>v\<^sub>a\<^sub>l \<sim> lo : sz\<^sub>m\<^sub>e\<^sub>m) (sz\<^sub>v\<^sub>a\<^sub>l - sz\<^sub>m\<^sub>e\<^sub>m) el\<rbrakk>
+            \<Longrightarrow> P mem w\<^sub>a\<^sub>d\<^sub>d\<^sub>r (Immediate w\<^sub>v\<^sub>a\<^sub>l) sz\<^sub>v\<^sub>a\<^sub>l el) \<close>
+
+      and \<open>(\<And>mem sz\<^sub>a\<^sub>d\<^sub>d\<^sub>r sz\<^sub>m\<^sub>e\<^sub>m w\<^sub>a\<^sub>d\<^sub>d\<^sub>r str sz sz\<^sub>v\<^sub>a\<^sub>l. \<lbrakk>type mem = Mem sz\<^sub>a\<^sub>d\<^sub>d\<^sub>r sz\<^sub>m\<^sub>e\<^sub>m; sz = sz\<^sub>v\<^sub>a\<^sub>l; sz\<^sub>m\<^sub>e\<^sub>m \<noteq> 0; sz\<^sub>m\<^sub>e\<^sub>m < sz\<^sub>v\<^sub>a\<^sub>l;
+             bits w\<^sub>a\<^sub>d\<^sub>d\<^sub>r = sz\<^sub>a\<^sub>d\<^sub>d\<^sub>r;
+             P mem[w\<^sub>a\<^sub>d\<^sub>d\<^sub>r \<leftarrow> (unknown[str]: Imm sz\<^sub>m\<^sub>e\<^sub>m), sz\<^sub>m\<^sub>e\<^sub>m] (succ w\<^sub>a\<^sub>d\<^sub>d\<^sub>r) (unknown[str]: Imm (sz\<^sub>v\<^sub>a\<^sub>l - sz\<^sub>m\<^sub>e\<^sub>m)) (sz\<^sub>v\<^sub>a\<^sub>l - sz\<^sub>m\<^sub>e\<^sub>m) en\<rbrakk>
+            \<Longrightarrow> P mem w\<^sub>a\<^sub>d\<^sub>d\<^sub>r (unknown[str]: (Imm sz)) sz\<^sub>v\<^sub>a\<^sub>l en) \<close>
+
+      and \<open>(\<And>mem sz\<^sub>a\<^sub>d\<^sub>d\<^sub>r sz\<^sub>m\<^sub>e\<^sub>m w\<^sub>a\<^sub>d\<^sub>d\<^sub>r sz v\<^sub>v\<^sub>a\<^sub>l sz\<^sub>v\<^sub>a\<^sub>l. \<lbrakk>type mem = Mem sz\<^sub>a\<^sub>d\<^sub>d\<^sub>r sz\<^sub>m\<^sub>e\<^sub>m; type v\<^sub>v\<^sub>a\<^sub>l = Imm sz; sz = sz\<^sub>v\<^sub>a\<^sub>l; sz\<^sub>v\<^sub>a\<^sub>l = sz\<^sub>m\<^sub>e\<^sub>m; sz\<^sub>m\<^sub>e\<^sub>m > 0; bits w\<^sub>a\<^sub>d\<^sub>d\<^sub>r = sz\<^sub>a\<^sub>d\<^sub>d\<^sub>r\<rbrakk>
+            \<Longrightarrow> P mem w\<^sub>a\<^sub>d\<^sub>d\<^sub>r v\<^sub>v\<^sub>a\<^sub>l sz\<^sub>v\<^sub>a\<^sub>l en)\<close>
+
+      (* Invalid cases *)
+      and \<open>(\<And>mem sz\<^sub>a\<^sub>d\<^sub>d\<^sub>r sz\<^sub>m\<^sub>e\<^sub>m w\<^sub>a\<^sub>d\<^sub>d\<^sub>r v\<^sub>v\<^sub>a\<^sub>l sz\<^sub>v\<^sub>a\<^sub>l. \<lbrakk>type mem = Mem sz\<^sub>a\<^sub>d\<^sub>d\<^sub>r sz\<^sub>m\<^sub>e\<^sub>m; bits w\<^sub>a\<^sub>d\<^sub>d\<^sub>r \<noteq> sz\<^sub>a\<^sub>d\<^sub>d\<^sub>r\<rbrakk>
+            \<Longrightarrow> P mem w\<^sub>a\<^sub>d\<^sub>d\<^sub>r v\<^sub>v\<^sub>a\<^sub>l sz\<^sub>v\<^sub>a\<^sub>l en)\<close>
+      and \<open>(\<And>mem sz\<^sub>a\<^sub>d\<^sub>d\<^sub>r sz\<^sub>m\<^sub>e\<^sub>m w\<^sub>a\<^sub>d\<^sub>d\<^sub>r v\<^sub>v\<^sub>a\<^sub>l sz\<^sub>v\<^sub>a\<^sub>l. \<lbrakk>type mem = Mem sz\<^sub>a\<^sub>d\<^sub>d\<^sub>r sz\<^sub>m\<^sub>e\<^sub>m; sz\<^sub>v\<^sub>a\<^sub>l < sz\<^sub>m\<^sub>e\<^sub>m\<rbrakk>
+            \<Longrightarrow> P mem w\<^sub>a\<^sub>d\<^sub>d\<^sub>r v\<^sub>v\<^sub>a\<^sub>l sz\<^sub>v\<^sub>a\<^sub>l en)\<close>
+      and \<open>(\<And>mem sz\<^sub>a\<^sub>d\<^sub>d\<^sub>r sz\<^sub>m\<^sub>e\<^sub>m w\<^sub>a\<^sub>d\<^sub>d\<^sub>r v\<^sub>v\<^sub>a\<^sub>l sz\<^sub>v\<^sub>a\<^sub>l. \<lbrakk>type mem = Mem sz\<^sub>a\<^sub>d\<^sub>d\<^sub>r sz\<^sub>m\<^sub>e\<^sub>m; sz\<^sub>m\<^sub>e\<^sub>m = 0\<rbrakk>
+            \<Longrightarrow> P mem w\<^sub>a\<^sub>d\<^sub>d\<^sub>r v\<^sub>v\<^sub>a\<^sub>l sz\<^sub>v\<^sub>a\<^sub>l en)\<close>
+      and \<open>(\<And>mem w\<^sub>a\<^sub>d\<^sub>d\<^sub>r v\<^sub>v\<^sub>a\<^sub>l sz sz\<^sub>v\<^sub>a\<^sub>l. \<lbrakk>type v\<^sub>v\<^sub>a\<^sub>l = Imm sz; sz \<noteq> sz\<^sub>v\<^sub>a\<^sub>l\<rbrakk>
+            \<Longrightarrow> P mem w\<^sub>a\<^sub>d\<^sub>d\<^sub>r v\<^sub>v\<^sub>a\<^sub>l sz\<^sub>v\<^sub>a\<^sub>l en)\<close>
+      and \<open>(\<And>mem sz uv uw ux. type mem = Imm sz \<Longrightarrow> P mem uv uw ux en)\<close>
+      and \<open>(\<And>uu uv v\<^sub>v\<^sub>a\<^sub>l sz\<^sub>a\<^sub>d\<^sub>d\<^sub>r sz\<^sub>m\<^sub>e\<^sub>m ux. type v\<^sub>v\<^sub>a\<^sub>l = Mem sz\<^sub>a\<^sub>d\<^sub>d\<^sub>r sz\<^sub>m\<^sub>e\<^sub>m \<Longrightarrow> P uu uv v\<^sub>v\<^sub>a\<^sub>l ux en)\<close>
+    shows \<open>P mem w\<^sub>a\<^sub>d\<^sub>d\<^sub>r v\<^sub>v\<^sub>a\<^sub>l sz\<^sub>v\<^sub>a\<^sub>l en\<close>
+  using assms type.simps apply (erule_tac store''_inducts)
+
+
+lemma store'_wf_inducts[consumes 4]:
+  assumes \<open>v' = store' mem w\<^sub>a\<^sub>d\<^sub>d\<^sub>r v\<^sub>v\<^sub>a\<^sub>l sz\<^sub>v\<^sub>a\<^sub>l en\<close>
+      and \<open>\<Gamma> \<turnstile> mem :: Mem sz\<^sub>a\<^sub>d\<^sub>d\<^sub>r sz\<^sub>m\<^sub>e\<^sub>m\<close>
+      and \<open>\<Gamma> \<turnstile> v\<^sub>v\<^sub>a\<^sub>l :: Imm sz\<^sub>v\<^sub>a\<^sub>l\<close>
+      and \<open>bits w\<^sub>a\<^sub>d\<^sub>d\<^sub>r = sz\<^sub>a\<^sub>d\<^sub>d\<^sub>r\<close>
+      and \<open>sz\<^sub>m\<^sub>e\<^sub>m dvd sz\<^sub>v\<^sub>a\<^sub>l\<close>
+      and \<open>(\<And>mem sz\<^sub>a\<^sub>d\<^sub>d\<^sub>r sz\<^sub>m\<^sub>e\<^sub>m w\<^sub>a\<^sub>d\<^sub>d\<^sub>r w\<^sub>v\<^sub>a\<^sub>l sz\<^sub>v\<^sub>a\<^sub>l. \<lbrakk>type mem = Mem sz\<^sub>a\<^sub>d\<^sub>d\<^sub>r sz\<^sub>m\<^sub>e\<^sub>m; bits w\<^sub>v\<^sub>a\<^sub>l = sz\<^sub>v\<^sub>a\<^sub>l; sz\<^sub>m\<^sub>e\<^sub>m \<noteq> 0; sz\<^sub>m\<^sub>e\<^sub>m < sz\<^sub>v\<^sub>a\<^sub>l;
+             bits w\<^sub>a\<^sub>d\<^sub>d\<^sub>r = sz\<^sub>a\<^sub>d\<^sub>d\<^sub>r;
+             P mem[w\<^sub>a\<^sub>d\<^sub>d\<^sub>r \<leftarrow> Immediate ext w\<^sub>v\<^sub>a\<^sub>l \<sim> hi : sz\<^sub>v\<^sub>a\<^sub>l \<sim> lo : sz\<^sub>v\<^sub>a\<^sub>l - sz\<^sub>m\<^sub>e\<^sub>m, sz\<^sub>m\<^sub>e\<^sub>m] (succ w\<^sub>a\<^sub>d\<^sub>d\<^sub>r) (Immediate ext w\<^sub>v\<^sub>a\<^sub>l \<sim> hi : sz\<^sub>v\<^sub>a\<^sub>l - sz\<^sub>m\<^sub>e\<^sub>m \<sim> lo : 0) (sz\<^sub>v\<^sub>a\<^sub>l - sz\<^sub>m\<^sub>e\<^sub>m) be\<rbrakk>
+            \<Longrightarrow> P mem w\<^sub>a\<^sub>d\<^sub>d\<^sub>r (Immediate w\<^sub>v\<^sub>a\<^sub>l) sz\<^sub>v\<^sub>a\<^sub>l be)\<close>
+
+      and \<open>(\<And>mem sz\<^sub>a\<^sub>d\<^sub>d\<^sub>r sz\<^sub>m\<^sub>e\<^sub>m w\<^sub>a\<^sub>d\<^sub>d\<^sub>r w\<^sub>v\<^sub>a\<^sub>l sz\<^sub>v\<^sub>a\<^sub>l. \<lbrakk>type mem = Mem sz\<^sub>a\<^sub>d\<^sub>d\<^sub>r sz\<^sub>m\<^sub>e\<^sub>m; bits w\<^sub>v\<^sub>a\<^sub>l = sz\<^sub>v\<^sub>a\<^sub>l; sz\<^sub>m\<^sub>e\<^sub>m \<noteq> 0; sz\<^sub>m\<^sub>e\<^sub>m < sz\<^sub>v\<^sub>a\<^sub>l;
+             bits w\<^sub>a\<^sub>d\<^sub>d\<^sub>r = sz\<^sub>a\<^sub>d\<^sub>d\<^sub>r;
+             P mem[w\<^sub>a\<^sub>d\<^sub>d\<^sub>r \<leftarrow> Immediate ext w\<^sub>v\<^sub>a\<^sub>l \<sim> hi : sz\<^sub>m\<^sub>e\<^sub>m \<sim> lo : 0, sz\<^sub>m\<^sub>e\<^sub>m] (succ w\<^sub>a\<^sub>d\<^sub>d\<^sub>r) (Immediate ext w\<^sub>v\<^sub>a\<^sub>l \<sim> hi : sz\<^sub>v\<^sub>a\<^sub>l \<sim> lo : sz\<^sub>m\<^sub>e\<^sub>m) (sz\<^sub>v\<^sub>a\<^sub>l - sz\<^sub>m\<^sub>e\<^sub>m) el\<rbrakk>
+            \<Longrightarrow> P mem w\<^sub>a\<^sub>d\<^sub>d\<^sub>r (Immediate w\<^sub>v\<^sub>a\<^sub>l) sz\<^sub>v\<^sub>a\<^sub>l el) \<close>
+
+      and \<open>(\<And>mem sz\<^sub>a\<^sub>d\<^sub>d\<^sub>r sz\<^sub>m\<^sub>e\<^sub>m w\<^sub>a\<^sub>d\<^sub>d\<^sub>r str sz sz\<^sub>v\<^sub>a\<^sub>l en. \<lbrakk>type mem = Mem sz\<^sub>a\<^sub>d\<^sub>d\<^sub>r sz\<^sub>m\<^sub>e\<^sub>m; sz = sz\<^sub>v\<^sub>a\<^sub>l; sz\<^sub>m\<^sub>e\<^sub>m \<noteq> 0; sz\<^sub>m\<^sub>e\<^sub>m < sz\<^sub>v\<^sub>a\<^sub>l;
+             bits w\<^sub>a\<^sub>d\<^sub>d\<^sub>r = sz\<^sub>a\<^sub>d\<^sub>d\<^sub>r;
+             P mem[w\<^sub>a\<^sub>d\<^sub>d\<^sub>r \<leftarrow> (unknown[str]: Imm sz\<^sub>m\<^sub>e\<^sub>m), sz\<^sub>m\<^sub>e\<^sub>m] (succ w\<^sub>a\<^sub>d\<^sub>d\<^sub>r) (unknown[str]: Imm (sz\<^sub>v\<^sub>a\<^sub>l - sz\<^sub>m\<^sub>e\<^sub>m)) (sz\<^sub>v\<^sub>a\<^sub>l - sz\<^sub>m\<^sub>e\<^sub>m) en\<rbrakk>
+            \<Longrightarrow> P mem w\<^sub>a\<^sub>d\<^sub>d\<^sub>r (unknown[str]: (Imm sz)) sz\<^sub>v\<^sub>a\<^sub>l en) \<close>
+
+      and \<open>(\<And>mem sz\<^sub>a\<^sub>d\<^sub>d\<^sub>r sz\<^sub>m\<^sub>e\<^sub>m w\<^sub>a\<^sub>d\<^sub>d\<^sub>r sz v\<^sub>v\<^sub>a\<^sub>l sz\<^sub>v\<^sub>a\<^sub>l en. \<lbrakk>type mem = Mem sz\<^sub>a\<^sub>d\<^sub>d\<^sub>r sz\<^sub>m\<^sub>e\<^sub>m; type v\<^sub>v\<^sub>a\<^sub>l = Imm sz; sz = sz\<^sub>v\<^sub>a\<^sub>l; sz\<^sub>v\<^sub>a\<^sub>l = sz\<^sub>m\<^sub>e\<^sub>m; sz\<^sub>m\<^sub>e\<^sub>m > 0; bits w\<^sub>a\<^sub>d\<^sub>d\<^sub>r = sz\<^sub>a\<^sub>d\<^sub>d\<^sub>r\<rbrakk>
+            \<Longrightarrow> P mem w\<^sub>a\<^sub>d\<^sub>d\<^sub>r v\<^sub>v\<^sub>a\<^sub>l sz\<^sub>v\<^sub>a\<^sub>l en)\<close>
+
+    shows \<open>P mem w\<^sub>a\<^sub>d\<^sub>d\<^sub>r v\<^sub>v\<^sub>a\<^sub>l sz\<^sub>v\<^sub>a\<^sub>l en\<close>
+  using assms(2) apply (drule_tac \<Gamma>_val_type)
+  using assms(2) apply (drule_tac typing_val_mem)
+  using assms(3) apply (drule_tac typing_val_imm)
+
+  using assms(1,5-9) apply (induct mem w\<^sub>a\<^sub>d\<^sub>d\<^sub>r v\<^sub>v\<^sub>a\<^sub>l sz\<^sub>v\<^sub>a\<^sub>l en rule: store''_inducts)
+  apply (auto simp del: extract_word.simps)
+  oops
+
+
+
+
+lemma store_wf_inducts[consumes 4]:
+  assumes \<open>v' = store mem w\<^sub>a\<^sub>d\<^sub>d\<^sub>r v\<^sub>v\<^sub>a\<^sub>l sz\<^sub>v\<^sub>a\<^sub>l en\<close>
+      and \<open>\<Gamma> \<turnstile> mem :: Mem sz\<^sub>a\<^sub>d\<^sub>d\<^sub>r sz\<^sub>m\<^sub>e\<^sub>m\<close>
+      and \<open>\<Gamma> \<turnstile> v\<^sub>v\<^sub>a\<^sub>l :: Imm sz\<^sub>v\<^sub>a\<^sub>l\<close>
+      and \<open>sz\<^sub>m\<^sub>e\<^sub>m dvd sz\<^sub>v\<^sub>a\<^sub>l\<close>
+      and \<open>\<And>w\<^sub>v\<^sub>a\<^sub>l. \<lbrakk>type mem = Mem sz\<^sub>a\<^sub>d\<^sub>d\<^sub>r sz\<^sub>m\<^sub>e\<^sub>m; sz\<^sub>m\<^sub>e\<^sub>m \<noteq> 0; sz\<^sub>v\<^sub>a\<^sub>l > sz\<^sub>m\<^sub>e\<^sub>m; 
+              v\<^sub>v\<^sub>a\<^sub>l = Immediate w\<^sub>v\<^sub>a\<^sub>l; en = be; v' = (
+            let 
+              w\<^sub>v\<^sub>a\<^sub>l\<^sub>_\<^sub>c\<^sub>o\<^sub>n\<^sub>c\<^sub>a\<^sub>t :: word = ext w\<^sub>v\<^sub>a\<^sub>l \<sim> hi : (sz\<^sub>v\<^sub>a\<^sub>l - sz\<^sub>m\<^sub>e\<^sub>m) \<sim> lo : 0;
+              w\<^sub>v\<^sub>a\<^sub>l\<^sub>_\<^sub>v\<^sub>a\<^sub>l :: word = ext w\<^sub>v\<^sub>a\<^sub>l \<sim> hi : sz\<^sub>v\<^sub>a\<^sub>l \<sim> lo : (sz\<^sub>v\<^sub>a\<^sub>l - sz\<^sub>m\<^sub>e\<^sub>m)
+            in
+              store (mem[w\<^sub>a\<^sub>d\<^sub>d\<^sub>r \<leftarrow> (Immediate w\<^sub>v\<^sub>a\<^sub>l\<^sub>_\<^sub>v\<^sub>a\<^sub>l), sz\<^sub>m\<^sub>e\<^sub>m]) (succ w\<^sub>a\<^sub>d\<^sub>d\<^sub>r) (Immediate w\<^sub>v\<^sub>a\<^sub>l\<^sub>_\<^sub>c\<^sub>o\<^sub>n\<^sub>c\<^sub>a\<^sub>t) (sz\<^sub>v\<^sub>a\<^sub>l - sz\<^sub>m\<^sub>e\<^sub>m) be)\<rbrakk> \<Longrightarrow> P mem w\<^sub>a\<^sub>d\<^sub>d\<^sub>r (Immediate w\<^sub>v\<^sub>a\<^sub>l) sz\<^sub>v\<^sub>a\<^sub>l be\<close>
+      and \<open>\<And>w\<^sub>v\<^sub>a\<^sub>l. \<lbrakk>type mem = Mem sz\<^sub>a\<^sub>d\<^sub>d\<^sub>r sz\<^sub>m\<^sub>e\<^sub>m; sz\<^sub>m\<^sub>e\<^sub>m \<noteq> 0; sz\<^sub>v\<^sub>a\<^sub>l > sz\<^sub>m\<^sub>e\<^sub>m; 
+              v\<^sub>v\<^sub>a\<^sub>l = Immediate w\<^sub>v\<^sub>a\<^sub>l; en = el; v' = (
+            let 
+              w\<^sub>v\<^sub>a\<^sub>l\<^sub>_\<^sub>c\<^sub>o\<^sub>n\<^sub>c\<^sub>a\<^sub>t :: word = ext w\<^sub>v\<^sub>a\<^sub>l \<sim> hi : sz\<^sub>v\<^sub>a\<^sub>l \<sim> lo : sz\<^sub>m\<^sub>e\<^sub>m;
+              w\<^sub>v\<^sub>a\<^sub>l\<^sub>_\<^sub>v\<^sub>a\<^sub>l :: word = ext w\<^sub>v\<^sub>a\<^sub>l \<sim> hi : sz\<^sub>m\<^sub>e\<^sub>m \<sim> lo : 0
+            in
+              store (mem[w\<^sub>a\<^sub>d\<^sub>d\<^sub>r \<leftarrow> (Immediate w\<^sub>v\<^sub>a\<^sub>l\<^sub>_\<^sub>v\<^sub>a\<^sub>l), sz\<^sub>m\<^sub>e\<^sub>m]) (succ w\<^sub>a\<^sub>d\<^sub>d\<^sub>r) (Immediate w\<^sub>v\<^sub>a\<^sub>l\<^sub>_\<^sub>c\<^sub>o\<^sub>n\<^sub>c\<^sub>a\<^sub>t) (sz\<^sub>v\<^sub>a\<^sub>l - sz\<^sub>m\<^sub>e\<^sub>m) el)\<rbrakk> \<Longrightarrow> P mem w\<^sub>a\<^sub>d\<^sub>d\<^sub>r (Immediate w\<^sub>v\<^sub>a\<^sub>l) sz\<^sub>v\<^sub>a\<^sub>l el\<close>
+      and \<open>\<And>str t. \<lbrakk>type mem = Mem sz\<^sub>a\<^sub>d\<^sub>d\<^sub>r sz\<^sub>m\<^sub>e\<^sub>m; sz\<^sub>m\<^sub>e\<^sub>m \<noteq> 0; sz\<^sub>v\<^sub>a\<^sub>l > sz\<^sub>m\<^sub>e\<^sub>m; v\<^sub>v\<^sub>a\<^sub>l = unknown[str]: t; v' = (
+            (store (mem[w\<^sub>a\<^sub>d\<^sub>d\<^sub>r \<leftarrow> (Unknown str (Imm sz\<^sub>m\<^sub>e\<^sub>m)), sz\<^sub>m\<^sub>e\<^sub>m]) (succ w\<^sub>a\<^sub>d\<^sub>d\<^sub>r) (unknown[str]: (Imm (sz\<^sub>v\<^sub>a\<^sub>l - sz\<^sub>m\<^sub>e\<^sub>m))) (sz\<^sub>v\<^sub>a\<^sub>l - sz\<^sub>m\<^sub>e\<^sub>m) en)
+        )\<rbrakk> \<Longrightarrow> P mem w\<^sub>a\<^sub>d\<^sub>d\<^sub>r v\<^sub>v\<^sub>a\<^sub>l sz\<^sub>v\<^sub>a\<^sub>l en\<close>
+      and \<open>\<lbrakk>type mem = Mem sz\<^sub>a\<^sub>d\<^sub>d\<^sub>r sz\<^sub>m\<^sub>e\<^sub>m; sz\<^sub>m\<^sub>e\<^sub>m = sz\<^sub>v\<^sub>a\<^sub>l; v' = (mem[w\<^sub>a\<^sub>d\<^sub>d\<^sub>r \<leftarrow> v\<^sub>v\<^sub>a\<^sub>l, sz\<^sub>m\<^sub>e\<^sub>m])\<rbrakk> \<Longrightarrow> P mem w\<^sub>a\<^sub>d\<^sub>d\<^sub>r v\<^sub>v\<^sub>a\<^sub>l sz\<^sub>v\<^sub>a\<^sub>l en\<close>
+    shows \<open>P mem w\<^sub>a\<^sub>d\<^sub>d\<^sub>r v\<^sub>v\<^sub>a\<^sub>l sz\<^sub>v\<^sub>a\<^sub>l en\<close>
+  using assms 
+  apply (frule_tac \<Gamma>_val_imm_not_storage)
+  apply (frule_tac \<Gamma>_val_mem_not_immediate)
+  apply (frule_tac typing_val_implies_valid_t)
+  apply (frule_tac t=\<open>Imm sz\<^sub>v\<^sub>a\<^sub>l\<close> in typing_val_implies_valid_t)
+  apply (cases mem)
+  apply presburger
+  apply (erule store_inducts)
+  apply (auto simp del: store.simps extract_word.simps)
+  apply (frule_tac typing_val_storage)
+  apply (erule store_inducts)
+  apply (auto simp del: store.simps extract_word.simps)
+  using assms(1) by blast+
+
+(*
+lemma \<open>\<Gamma> \<turnstile> v :: Mem sz\<^sub>a\<^sub>d\<^sub>d\<^sub>r sz\<^sub>m\<^sub>e\<^sub>m \<Longrightarrow>
+       \<Gamma> \<turnstile> v' :: Imm sz\<^sub>v\<^sub>a\<^sub>l \<Longrightarrow>
+       bits w\<^sub>a\<^sub>d\<^sub>d\<^sub>r = sz\<^sub>a\<^sub>d\<^sub>d\<^sub>r \<Longrightarrow>
+       0 < sz\<^sub>m\<^sub>e\<^sub>m \<Longrightarrow> sz\<^sub>m\<^sub>e\<^sub>m \<le> sz\<^sub>v\<^sub>a\<^sub>l \<Longrightarrow> 
+*)
+lemma XXXXXX:
+  assumes \<open>v' = store' mem w\<^sub>a\<^sub>d\<^sub>d\<^sub>r v\<^sub>v\<^sub>a\<^sub>l sz\<^sub>v\<^sub>a\<^sub>l en\<close>
+      and \<open>\<Gamma> \<turnstile> mem :: (Mem sz\<^sub>a\<^sub>d\<^sub>d\<^sub>r sz\<^sub>m\<^sub>e\<^sub>m)\<close>
+      and \<open>\<Gamma> \<turnstile> v\<^sub>v\<^sub>a\<^sub>l :: (Imm sz\<^sub>v\<^sub>a\<^sub>l)\<close>
+      and \<open>sz\<^sub>m\<^sub>e\<^sub>m dvd sz\<^sub>v\<^sub>a\<^sub>l\<close>
+      and \<open>bits w\<^sub>a\<^sub>d\<^sub>d\<^sub>r = sz\<^sub>a\<^sub>d\<^sub>d\<^sub>r\<close>
+    shows \<open>\<Gamma> \<turnstile> v' :: (Mem sz\<^sub>a\<^sub>d\<^sub>d\<^sub>r sz\<^sub>m\<^sub>e\<^sub>m)\<close>
+  oops
+
+
+lemma store: 
+  assumes \<open>type v = Mem sz\<^sub>a\<^sub>d\<^sub>d\<^sub>r sz\<^sub>v\<^sub>a\<^sub>l\<close> and \<open>sz\<^sub>v\<^sub>a\<^sub>l > 0\<close>
+    shows \<open>v[w \<leftarrow> v', sz\<^sub>v\<^sub>a\<^sub>l] = store v w v' sz\<^sub>v\<^sub>a\<^sub>l en\<close>
+  using assms by auto
+
+lemma store_be: 
+  assumes \<open>type v = Mem sz\<^sub>a\<^sub>d\<^sub>d\<^sub>r sz\<^sub>v\<^sub>a\<^sub>l\<close> and \<open>sz\<^sub>v\<^sub>a\<^sub>l < sz\<close> and \<open>0 < sz\<^sub>v\<^sub>a\<^sub>l\<close>
+      and \<open>w\<^sub>1 = ext w\<^sub>v\<^sub>a\<^sub>l \<sim> hi : sz \<sim> lo : (sz - sz\<^sub>v\<^sub>a\<^sub>l)\<close>
+      and \<open>w\<^sub>2 = ext w\<^sub>v\<^sub>a\<^sub>l \<sim> hi : (sz - sz\<^sub>v\<^sub>a\<^sub>l) \<sim> lo : 0\<close>
+      and \<open>v' = store v w\<^sub>a\<^sub>d\<^sub>d\<^sub>r (Immediate w\<^sub>1) sz\<^sub>v\<^sub>a\<^sub>l be\<close>
+      and \<open>v'' = store v' (succ w\<^sub>a\<^sub>d\<^sub>d\<^sub>r) (Immediate w\<^sub>2) (sz - sz\<^sub>v\<^sub>a\<^sub>l) be\<close>
+    shows \<open>v'' = store v w\<^sub>a\<^sub>d\<^sub>d\<^sub>r (Immediate w\<^sub>v\<^sub>a\<^sub>l) sz be\<close>
+  using assms apply (simp del: extract_word.simps)
+  by metis+
+
+lemma store_el: 
+  assumes \<open>type v = Mem sz\<^sub>a\<^sub>d\<^sub>d\<^sub>r sz\<^sub>v\<^sub>a\<^sub>l\<close> and \<open>sz\<^sub>v\<^sub>a\<^sub>l < sz\<close> and \<open>0 < sz\<^sub>v\<^sub>a\<^sub>l\<close>
+      and \<open>w\<^sub>1 = ext w\<^sub>v\<^sub>a\<^sub>l \<sim> hi : sz\<^sub>v\<^sub>a\<^sub>l \<sim> lo : 0\<close>
+      and \<open>w\<^sub>2 = ext w\<^sub>v\<^sub>a\<^sub>l \<sim> hi : sz \<sim> lo : sz\<^sub>v\<^sub>a\<^sub>l\<close>
+      and \<open>v' = store v w\<^sub>a\<^sub>d\<^sub>d\<^sub>r (Immediate w\<^sub>1) sz\<^sub>v\<^sub>a\<^sub>l el\<close>
+      and \<open>v'' = store v' (succ w\<^sub>a\<^sub>d\<^sub>d\<^sub>r) (Immediate w\<^sub>2) (sz - sz\<^sub>v\<^sub>a\<^sub>l) el\<close>
+    shows \<open>v'' = store v w\<^sub>a\<^sub>d\<^sub>d\<^sub>r (Immediate w\<^sub>v\<^sub>a\<^sub>l) sz el\<close>
+  using assms apply (simp del: extract_word.simps)
+  by metis+
+
+
+subsubsection \<open>Expression evaluation\<close>
 
 fun
-  store_val_be :: \<open>val \<Rightarrow> nat \<Rightarrow> word \<Rightarrow> val \<Rightarrow> nat \<Rightarrow> val\<close>
-where 
-  \<open>store_val_be mem sz\<^sub>m\<^sub>e\<^sub>m w\<^sub>a\<^sub>d\<^sub>d\<^sub>r v\<^sub>v\<^sub>a\<^sub>l sz\<^sub>v\<^sub>a\<^sub>l = (
-    if sz\<^sub>m\<^sub>e\<^sub>m > 0 \<and> sz\<^sub>v\<^sub>a\<^sub>l > sz\<^sub>m\<^sub>e\<^sub>m then
-      let sz\<^sub>v\<^sub>a\<^sub>l' :: nat = (sz\<^sub>v\<^sub>a\<^sub>l - sz\<^sub>m\<^sub>e\<^sub>m) in 
-      let w\<^sub>a\<^sub>d\<^sub>d\<^sub>r' :: word = succ w\<^sub>a\<^sub>d\<^sub>d\<^sub>r in
-      case v\<^sub>v\<^sub>a\<^sub>l of Immediate w\<^sub>v\<^sub>a\<^sub>l \<Rightarrow> (
-        let w\<^sub>v\<^sub>a\<^sub>l\<^sub>_\<^sub>c\<^sub>o\<^sub>n\<^sub>c\<^sub>a\<^sub>t :: word = ext w\<^sub>v\<^sub>a\<^sub>l \<sim> hi : sz\<^sub>v\<^sub>a\<^sub>l' \<sim> lo : 0 in
-        let w\<^sub>v\<^sub>a\<^sub>l\<^sub>_\<^sub>v\<^sub>a\<^sub>l :: word = ext w\<^sub>v\<^sub>a\<^sub>l \<sim> hi : sz\<^sub>v\<^sub>a\<^sub>l \<sim> lo : sz\<^sub>v\<^sub>a\<^sub>l' in
-        let mem' :: val = store_val_be mem sz\<^sub>m\<^sub>e\<^sub>m w\<^sub>a\<^sub>d\<^sub>d\<^sub>r' (Immediate w\<^sub>v\<^sub>a\<^sub>l\<^sub>_\<^sub>c\<^sub>o\<^sub>n\<^sub>c\<^sub>a\<^sub>t) sz\<^sub>v\<^sub>a\<^sub>l' in
-          (store_val mem' w\<^sub>a\<^sub>d\<^sub>d\<^sub>r (Immediate w\<^sub>v\<^sub>a\<^sub>l\<^sub>_\<^sub>v\<^sub>a\<^sub>l) sz\<^sub>m\<^sub>e\<^sub>m)
-      ) | Unknown str t \<Rightarrow> (
-        let mem' :: val = store_val_be mem sz\<^sub>m\<^sub>e\<^sub>m w\<^sub>a\<^sub>d\<^sub>d\<^sub>r' (Unknown str (Imm sz\<^sub>v\<^sub>a\<^sub>l')) sz\<^sub>v\<^sub>a\<^sub>l' in
-          (store_val mem' w\<^sub>a\<^sub>d\<^sub>d\<^sub>r (Unknown str (Imm sz\<^sub>m\<^sub>e\<^sub>m)) sz\<^sub>m\<^sub>e\<^sub>m)
-      )
-    else
-      store_val mem w\<^sub>a\<^sub>d\<^sub>d\<^sub>r v\<^sub>v\<^sub>a\<^sub>l sz\<^sub>m\<^sub>e\<^sub>m
-  )\<close>
-
-fun
-  store_val_el :: \<open>val \<Rightarrow> nat \<Rightarrow> word \<Rightarrow> val \<Rightarrow> nat \<Rightarrow> val\<close>
-where 
-  \<open>store_val_el mem sz\<^sub>m\<^sub>e\<^sub>m w\<^sub>a\<^sub>d\<^sub>d\<^sub>r v\<^sub>v\<^sub>a\<^sub>l sz\<^sub>v\<^sub>a\<^sub>l = (
-    if sz\<^sub>m\<^sub>e\<^sub>m > 0 \<and> sz\<^sub>v\<^sub>a\<^sub>l > sz\<^sub>m\<^sub>e\<^sub>m then
-      let sz\<^sub>v\<^sub>a\<^sub>l' :: nat = (sz\<^sub>v\<^sub>a\<^sub>l - sz\<^sub>m\<^sub>e\<^sub>m) in
-      let w\<^sub>a\<^sub>d\<^sub>d\<^sub>r' :: word = succ w\<^sub>a\<^sub>d\<^sub>d\<^sub>r in
-      case v\<^sub>v\<^sub>a\<^sub>l of Immediate w\<^sub>v\<^sub>a\<^sub>l \<Rightarrow> (
-        let w\<^sub>v\<^sub>a\<^sub>l\<^sub>_\<^sub>c\<^sub>o\<^sub>n\<^sub>c\<^sub>a\<^sub>t :: word = ext w\<^sub>v\<^sub>a\<^sub>l \<sim> hi : sz\<^sub>v\<^sub>a\<^sub>l \<sim> lo : sz\<^sub>m\<^sub>e\<^sub>m in
-        let w\<^sub>v\<^sub>a\<^sub>l\<^sub>_\<^sub>v\<^sub>a\<^sub>l :: word = ext w\<^sub>v\<^sub>a\<^sub>l \<sim> hi : sz\<^sub>m\<^sub>e\<^sub>m \<sim> lo : 0 in
-        let mem' :: val = store_val_el mem sz\<^sub>m\<^sub>e\<^sub>m w\<^sub>a\<^sub>d\<^sub>d\<^sub>r' (Immediate w\<^sub>v\<^sub>a\<^sub>l\<^sub>_\<^sub>c\<^sub>o\<^sub>n\<^sub>c\<^sub>a\<^sub>t) sz\<^sub>v\<^sub>a\<^sub>l' in
-          (store_val mem' w\<^sub>a\<^sub>d\<^sub>d\<^sub>r (Immediate w\<^sub>v\<^sub>a\<^sub>l\<^sub>_\<^sub>v\<^sub>a\<^sub>l) sz\<^sub>m\<^sub>e\<^sub>m)
-      ) | Unknown str t \<Rightarrow> (
-        let mem' :: val = store_val_be mem sz\<^sub>m\<^sub>e\<^sub>m w\<^sub>a\<^sub>d\<^sub>d\<^sub>r' (Unknown str (Imm sz\<^sub>v\<^sub>a\<^sub>l')) sz\<^sub>v\<^sub>a\<^sub>l' in
-          (store_val mem' w\<^sub>a\<^sub>d\<^sub>d\<^sub>r (Unknown str (Imm sz\<^sub>m\<^sub>e\<^sub>m)) sz\<^sub>m\<^sub>e\<^sub>m)
-      )
-    else 
-      store_val mem w\<^sub>a\<^sub>d\<^sub>d\<^sub>r v\<^sub>v\<^sub>a\<^sub>l sz\<^sub>m\<^sub>e\<^sub>m
-  )\<close>
-
-fun
-  store_val_en :: \<open>val \<Rightarrow> nat \<Rightarrow> word \<Rightarrow> val \<Rightarrow> nat \<Rightarrow> Endian \<Rightarrow> val\<close>
-where 
-  \<open>store_val_en mem sz\<^sub>m\<^sub>e\<^sub>m w\<^sub>a\<^sub>d\<^sub>d\<^sub>r v\<^sub>v\<^sub>a\<^sub>l sz\<^sub>v\<^sub>a\<^sub>l be = store_val_be mem sz\<^sub>m\<^sub>e\<^sub>m w\<^sub>a\<^sub>d\<^sub>d\<^sub>r v\<^sub>v\<^sub>a\<^sub>l sz\<^sub>v\<^sub>a\<^sub>l\<close> |
-  \<open>store_val_en mem sz\<^sub>m\<^sub>e\<^sub>m w\<^sub>a\<^sub>d\<^sub>d\<^sub>r v\<^sub>v\<^sub>a\<^sub>l sz\<^sub>v\<^sub>a\<^sub>l el = store_val_el mem sz\<^sub>m\<^sub>e\<^sub>m w\<^sub>a\<^sub>d\<^sub>d\<^sub>r v\<^sub>v\<^sub>a\<^sub>l sz\<^sub>v\<^sub>a\<^sub>l\<close>
- 
-
-function
   eval_exp :: \<open>variables \<Rightarrow> exp \<Rightarrow> val\<close>
 where
   \<open>eval_exp \<Delta> (Val v) = v\<close> |
@@ -147,7 +592,7 @@ where
         Unsigned \<Rightarrow> Immediate (ext w \<sim> hi : (sz - 1) \<sim> lo : 0)) |
       Unknown str t \<Rightarrow> Unknown str (Imm sz)
   )\<close> |
-  \<open>eval_exp \<Delta> (Let var e\<^sub>1 e\<^sub>2) = (eval_exp \<Delta> ([(eval_exp \<Delta> e\<^sub>1)\<sslash>var] e\<^sub>2))\<close> |
+  \<open>eval_exp \<Delta> (Let var e\<^sub>1 e\<^sub>2) = (eval_exp (\<Delta> (var \<mapsto> (eval_exp \<Delta> e\<^sub>1))) e\<^sub>2)\<close> |
   \<open>eval_exp \<Delta> (Ite e\<^sub>1 e\<^sub>2 e\<^sub>3) = (
     let v\<^sub>1 = eval_exp \<Delta> e\<^sub>1 in
     let v\<^sub>2 = eval_exp \<Delta> e\<^sub>2 in
@@ -180,7 +625,7 @@ where
     let v\<^sub>1 = eval_exp \<Delta> e\<^sub>1 in 
     case v\<^sub>1 of Storage v w v' sz\<^sub>m\<^sub>e\<^sub>m \<Rightarrow> (
       case v\<^sub>2 of Immediate w\<^sub>a\<^sub>d\<^sub>d\<^sub>r \<Rightarrow> (
-        load_val_en v\<^sub>1 sz\<^sub>m\<^sub>e\<^sub>m w\<^sub>a\<^sub>d\<^sub>d\<^sub>r sz\<^sub>v\<^sub>a\<^sub>l ed
+        load v\<^sub>1 w\<^sub>a\<^sub>d\<^sub>d\<^sub>r sz\<^sub>v\<^sub>a\<^sub>l ed
       ) | Unknown str _ \<Rightarrow> Unknown str (Imm sz\<^sub>v\<^sub>a\<^sub>l)
     ) | Unknown str _ \<Rightarrow> Unknown str (Imm sz\<^sub>v\<^sub>a\<^sub>l)
   )\<close> |
@@ -191,12 +636,10 @@ where
     let t = type v\<^sub>1 in
     case v\<^sub>2 of Immediate w\<^sub>a\<^sub>d\<^sub>d\<^sub>r \<Rightarrow> (
       case t of Mem _ sz\<^sub>m\<^sub>e\<^sub>m \<Rightarrow> (
-        store_val_en v\<^sub>1 sz\<^sub>m\<^sub>e\<^sub>m w\<^sub>a\<^sub>d\<^sub>d\<^sub>r v\<^sub>3 sz\<^sub>v\<^sub>a\<^sub>l ed)
+        store v\<^sub>1 w\<^sub>a\<^sub>d\<^sub>d\<^sub>r v\<^sub>3 sz\<^sub>v\<^sub>a\<^sub>l ed)
     ) | Unknown str _ \<Rightarrow> Unknown str t
   )\<close>
-  apply auto
-  by (metis old.prod.exhaust wfe.cases)
-
+(*
 lemma let_substitute_Let_size_less: 
     \<open>size_class.size (Let var e\<^sub>1 e\<^sub>2) > size_class.size ([(eval_exp \<Delta> e\<^sub>1)\<sslash>var] e\<^sub>2)\<close>
   apply auto
@@ -209,21 +652,43 @@ termination eval_exp
   apply (relation \<open>(\<lambda>p. size_class.size (snd p)) <*mlex*> {}\<close>)
   apply (auto simp add: wf_mlex mlex_prod_def)
   using let_substitute_Let_size_less by simp
+*)
 
 fun 
   step_pred_exp :: \<open>variables \<Rightarrow> exp \<Rightarrow> exp \<Rightarrow> bool\<close> (\<open>_ \<turnstile> _ \<leadsto> _\<close>)
 where
   \<open>(_ \<turnstile> (Val v) \<leadsto> _) = False\<close> |
-  \<open>(\<Delta> \<turnstile> e \<leadsto> e') = (eval_exp \<Delta> e = eval_exp \<Delta> e')\<close>
+  \<open>(\<Delta> \<turnstile> e \<leadsto> e') = (
+    e \<noteq> e' \<and>
+    eval_exp \<Delta> e = eval_exp \<Delta> e'
+  )\<close>
+(*    size_class.size e \<ge> size_class.size e' \<and> *)
 
 
-lemma VAL_NO_STEP: \<open>\<not>(\<Delta> \<turnstile> (Val v) \<leadsto> e')\<close>
+lemma STEP_NOT_EQ: \<open>\<not>(\<Delta> \<turnstile> e \<leadsto> e)\<close>
+  by (induct e, auto)
+
+lemma STEP_NOT_REDUCTION: 
+  assumes \<open>eval_exp \<Delta> e \<noteq> eval_exp \<Delta> e'\<close>
+    shows \<open>\<not>(\<Delta> \<turnstile> e \<leadsto> e')\<close>
+  using assms by (induct e, auto)
+
+lemma STEP_NOT_VAL: \<open>\<not>(\<Delta> \<turnstile> (Val v) \<leadsto> e')\<close>
   by simp
 
-lemma STEP_NOT_VAL: 
-  assumes \<open>(\<Delta> \<turnstile> e \<leadsto> e')\<close>
+lemma STEP_IMPLIES_NOT_VAL: 
+  assumes \<open>\<Delta> \<turnstile> e \<leadsto> e'\<close>
     shows \<open>e \<noteq> Val v\<close>
   using assms by auto
+
+lemma STEP_NEXT: 
+  assumes \<open>eval_exp \<Delta> e = eval_exp \<Delta> e'\<close>
+      and \<open>e \<noteq> e'\<close> and \<open>\<forall>v. e \<noteq> Val v\<close>
+      and \<open>size_class.size e \<ge> size_class.size e'\<close> 
+    shows \<open>\<Delta> \<turnstile> e \<leadsto> e'\<close>
+  using assms by (induct e, auto)
+
+
 
 lemma VAR_IN:
   assumes \<open>(var, v) \<in>\<^sub>\<Delta> \<Delta>\<close>
@@ -264,12 +729,15 @@ lemma LOAD_UN_ADDR: \<open>\<Delta> \<turnstile> (Load (Val (Storage v w\<^sub>1
   by auto
 
 lemma LOAD_WORD_BE:
-  assumes \<open>sz' > sz\<close> and \<open>sz \<noteq> 0\<close> and \<open>succ w = w'\<close> and \<open>type v = (Mem sasas sz)\<close> 
+  assumes \<open>sz' > sz\<close> and \<open>sz > 0\<close> and \<open>succ w = w'\<close> and \<open>type v = (Mem sz\<^sub>a\<^sub>d\<^sub>d\<^sub>r sz)\<close> 
     shows \<open>\<Delta> \<turnstile> (Load (Val v) (Val (Immediate w)) be sz') \<leadsto> (Concat (Load (Val v) (Val (Immediate w)) be sz) ((Load (Val v) (Val (Immediate w')) be (sz' - sz))))\<close> 
   apply (auto simp only: step_pred_exp.simps eval_exp.simps Let_def)
-  apply (cases v, auto)
-  using assms(4) apply auto
-  apply (metis Suc_leD Suc_leI assms(1) le_add_diff_inverse)
+  apply (cases v)
+  using assms(4) apply auto[1]
+  subgoal
+    using assms(1-2) by (simp del: load.simps)
+  subgoal
+    using assms(4) load_mem_simps apply (frule_tac w\<^sub>a\<^sub>d\<^sub>d\<^sub>r=w and sz\<^sub>v\<^sub>a\<^sub>l=sz and en=be in load_mem_simps)
   oops
 
 
@@ -294,23 +762,36 @@ lemma STORE_STEP_MEM:
   using assms by (cases e\<^sub>1, auto) 
 
 lemma STORE_WORD_BE:
-  assumes \<open>sz' > sz\<close> and \<open>succ w = w'\<close> and \<open>type v = Mem sz\<^sub>a\<^sub>d\<^sub>d\<^sub>r sz\<^sub>m\<^sub>e\<^sub>m\<close> 
-      and \<open>e\<^sub>1 = (Store (Val v) (Val (Immediate w)) be sz (Cast High sz (Val val)))\<close>
-    shows \<open>\<Delta> \<turnstile> (Store (Val v) (Val (Immediate w)) be sz' (Val val)) \<leadsto> (Store e\<^sub>1 (Val (Immediate w')) be (sz' - sz) (Cast Low (sz' - sz) (Val val)))\<close> 
+  assumes \<open>sz > sz\<^sub>m\<^sub>e\<^sub>m\<close> and \<open>succ w = w'\<close> and \<open>type v = Mem sz\<^sub>a\<^sub>d\<^sub>d\<^sub>r sz\<^sub>m\<^sub>e\<^sub>m\<close> 
+      and \<open>e\<^sub>1 = (Store (Val v) (Val (Immediate w)) be sz\<^sub>m\<^sub>e\<^sub>m (Cast High sz\<^sub>m\<^sub>e\<^sub>m (Val val)))\<close>
+    shows \<open>\<Delta> \<turnstile> (Store (Val v) (Val (Immediate w)) be sz (Val val)) \<leadsto> (Store e\<^sub>1 (Val (Immediate w')) be (sz - sz\<^sub>m\<^sub>e\<^sub>m) (Cast Low (sz - sz\<^sub>m\<^sub>e\<^sub>m) (Val val)))\<close>
+  apply (simp only: step_pred_exp.simps)
+  apply (intro conjI)
+  apply auto
+  using assms(3, 4) 
+  apply (simp add: Let_def del: store.simps)
+  apply (cases val)
+  apply (simp del: store.simps)
+  apply (subgoal_tac \<open>\<And>x sz\<^sub>m\<^sub>e\<^sub>m'. type
+                 (store v w
+                   (Immediate
+                     raw_val x1 \<Colon> Suc (bits x1 - Suc (bits x1 - sz\<^sub>m\<^sub>e\<^sub>m)))
+                   sz\<^sub>m\<^sub>e\<^sub>m be) =
+           Mem x sz\<^sub>m\<^sub>e\<^sub>m'\<close>)
+  using Type.inject(2) apply presburger
   oops
 
 lemma STORE_WORD_EL:
   assumes \<open>sz' > sz\<^sub>m\<^sub>e\<^sub>m\<close> and \<open>sz\<^sub>m\<^sub>e\<^sub>m > 0\<close> and \<open>succ w = w'\<close> and \<open>type v = Mem sz\<^sub>a\<^sub>d\<^sub>d\<^sub>r sz\<^sub>m\<^sub>e\<^sub>m\<close> 
       and \<open>e\<^sub>1 = (Store (Val v) (Val (Immediate w)) el sz\<^sub>m\<^sub>e\<^sub>m (Cast Low sz\<^sub>m\<^sub>e\<^sub>m (Val val)))\<close>
     shows \<open>\<Delta> \<turnstile> (Store (Val v) (Val (Immediate w)) el sz' (Val val)) \<leadsto> (Store e\<^sub>1 (Val (Immediate w')) el (sz' - sz\<^sub>m\<^sub>e\<^sub>m) (Cast High (sz' - sz\<^sub>m\<^sub>e\<^sub>m) (Val val)))\<close>
+  apply (simp only: step_pred_exp.simps)
   oops
 
 lemma STORE_VAL:
-  assumes \<open>type v = Mem sz\<^sub>a\<^sub>d\<^sub>d\<^sub>r sz\<^sub>m\<^sub>e\<^sub>m\<close>
+  assumes \<open>type v = Mem sz\<^sub>a\<^sub>d\<^sub>d\<^sub>r sz\<^sub>m\<^sub>e\<^sub>m\<close> and \<open>sz\<^sub>m\<^sub>e\<^sub>m > 0\<close>
     shows \<open>\<Delta> \<turnstile> (Store (Val v) (Val (Immediate w)) ed sz\<^sub>m\<^sub>e\<^sub>m (Val v')) \<leadsto> (Val (Storage v w v' sz\<^sub>m\<^sub>e\<^sub>m))\<close>
-  using assms apply (cases ed, auto)
-  by (auto simp add: store_val_def)
-
+  using assms by (cases ed, auto)
 
 
 lemma STORE_UN_ADDR:
@@ -324,8 +805,39 @@ lemma LET_STEP:
     shows \<open>\<Delta> \<turnstile> (Let var e\<^sub>1 e\<^sub>2) \<leadsto> (Let var e\<^sub>1' e\<^sub>2)\<close>
   using assms by (cases e\<^sub>1, auto)
 
-lemma LET: \<open>\<Delta> \<turnstile> (Let var (Val v\<^sub>1) e\<^sub>2) \<leadsto> ([(Val v\<^sub>1)\<sslash>var]e\<^sub>2)\<close>
-  by (simp add: let_substitue_val_exp_val_eq)
+fun 
+  capture_avoiding :: \<open>(Id \<times> Type) set \<Rightarrow> exp \<Rightarrow> bool\<close>
+where
+  \<open>capture_avoiding \<Delta> (Let var e\<^sub>1 e\<^sub>2) = (var \<notin> \<Delta> \<and> capture_avoiding \<Delta> e\<^sub>1 \<and> capture_avoiding (\<Delta> \<union> {var}) e\<^sub>2)\<close> |
+  \<open>capture_avoiding \<Delta> (UnOp _ e) = capture_avoiding \<Delta> e\<close> |
+  \<open>capture_avoiding \<Delta> (BinOp e\<^sub>1 _ e\<^sub>2) = (capture_avoiding \<Delta> e\<^sub>1 \<and> capture_avoiding \<Delta> e\<^sub>2)\<close> |
+  \<open>capture_avoiding \<Delta> (Cast _ _ e) = capture_avoiding \<Delta> e\<close> |
+  \<open>capture_avoiding \<Delta> (Ite e\<^sub>1 e\<^sub>2 e\<^sub>3) = (capture_avoiding \<Delta> e\<^sub>1 \<and> capture_avoiding \<Delta> e\<^sub>2 \<and> capture_avoiding \<Delta> e\<^sub>3)\<close> |
+  \<open>capture_avoiding \<Delta> (Extract _ _ e) = capture_avoiding \<Delta> e\<close> |
+  \<open>capture_avoiding \<Delta> (Concat e\<^sub>1 e\<^sub>2) = (capture_avoiding \<Delta> e\<^sub>1 \<and> capture_avoiding \<Delta> e\<^sub>2)\<close> |
+  \<open>capture_avoiding \<Delta> (Load e\<^sub>1 e\<^sub>2 _ _) = (capture_avoiding \<Delta> e\<^sub>1 \<and> capture_avoiding \<Delta> e\<^sub>2)\<close> |
+  \<open>capture_avoiding \<Delta> (Store e\<^sub>1 e\<^sub>2 _ _ e\<^sub>3) = (capture_avoiding \<Delta> e\<^sub>1 \<and> capture_avoiding \<Delta> e\<^sub>2 \<and> capture_avoiding \<Delta> e\<^sub>3)\<close> |
+  \<open>capture_avoiding _ _ = True\<close>
+
+lemma let_substitute_v_Let_size_less: 
+    \<open>size_class.size (Let var (Val v\<^sub>1) e\<^sub>2) > size_class.size ([v\<^sub>1\<sslash>var]e\<^sub>2)\<close>
+  by (induct e\<^sub>2, auto)
+
+lemma capture_avoiding_substitution_eval_eq:
+  assumes \<open>capture_avoiding (dom (\<Delta>(var \<mapsto> v))) e\<close> 
+    shows \<open>eval_exp (\<Delta>(var \<mapsto> v)) e = eval_exp \<Delta> ([v\<sslash>var]e)\<close> 
+  using assms apply (induct e arbitrary: \<Delta>)
+  apply auto
+  apply (simp_all only: let_substitute_val.simps capture_avoiding.simps)
+  by (metis dom_fun_upd fun_upd_twist option.distinct(1))
+
+lemma LET: 
+  assumes \<open>capture_avoiding (dom \<Delta>) (Let var (Val v\<^sub>1) e\<^sub>2)\<close>
+    shows \<open>\<Delta> \<turnstile> (Let var (Val v\<^sub>1) e\<^sub>2) \<leadsto> ([v\<^sub>1\<sslash>var]e\<^sub>2)\<close>
+  using assms apply auto
+  apply (metis less_not_refl let_substitute_v_Let_size_less)
+  using let_substitute_val_size_eq apply auto[1]
+  using capture_avoiding_substitution_eval_eq by simp
 
 lemma ITE_STEP_COND:
   assumes \<open>\<Delta> \<turnstile> e\<^sub>1 \<leadsto> e\<^sub>1'\<close>
@@ -340,10 +852,10 @@ lemma ITE_STEP_THEN:
 lemma ITE_STEP_ELSE:
   assumes \<open>\<Delta> \<turnstile> e\<^sub>3 \<leadsto> e\<^sub>3'\<close>
     shows \<open>\<Delta> \<turnstile> (Ite e\<^sub>1 e\<^sub>2 e\<^sub>3) \<leadsto> (Ite e\<^sub>1 e\<^sub>2 e\<^sub>3')\<close>
-  using assms apply (auto simp add: Let_def)
-  apply (cases \<open>eval_exp \<Delta> e\<^sub>1\<close>, auto)
-  by (cases e\<^sub>3, auto)
-  
+  using assms apply (cases e\<^sub>3, auto)
+  apply (metis STEP_NOT_REDUCTION assms)
+  using eval_exp.simps by presburger+
+
 
 lemma ITE_TRUE: \<open>\<Delta> \<turnstile> (Ite (Val (Immediate true)) (Val v\<^sub>2) (Val v\<^sub>3)) \<leadsto> (Val v\<^sub>2)\<close>
   by auto
